Add helpers

src/safety/Markers.v
@@ -128,6 +128,35 @@ Proof.
     end.
 Qed.
 
+Lemma handle_typing_inv_for_markers : forall Γ E_tag n_beta Ts T_B T_R op_body body T,
+  Γ ⊢ₜ term_handle E_tag n_beta Ts T_B T_R op_body body : T ->
+  exists n_α sig ret sig_β ret_β,
+    ctx_lookup_eff Γ E_tag = Some (n_α, n_beta, sig, ret) /\
+    List.length Ts = n_α /\ types_wf Γ Ts /\
+    ty_wf Γ T_B /\ ty_wf Γ T_R /\ no_local_ty_G Γ T_B = true /\ Γ ⊢ T_B <:: T_R /\
+    sig_β = inst_op_alpha n_α Ts n_beta sig /\
+    ret_β = inst_op_alpha n_α Ts n_beta ret /\
+    (bind_tm sig_β
+      :: bind_tm (type_fun ret_β lt_local (shift_ty n_beta 0 T_R))
+      :: push_ty_vars n_beta any_at_free Γ)
+      ⊢ₜ op_body : shift_ty n_beta 0 T_R /\
+    (bind_tm (type_ctor E_tag lt_local Ts) :: Γ) ⊢ₜ body : T_B /\
+    Γ ⊢ T_R <:: T.
+Proof.
+  intros Γ E_tag n_beta Ts T_B T_R op_body body T H.
+  remember (term_handle E_tag n_beta Ts T_B T_R op_body body) as s eqn:Hs.
+  induction H; try discriminate Hs.
+  - destruct (IHtyping Hs) as
+      (n_α & sig & ret & sig_β & ret_β & Heff & HlenTs & HwfTs & HwfTB & HwfTR
+       & Hnl & Hbr & Hsigβ & Hretβ & Hop & Hbody & Hsub).
+    exists n_α, sig, ret, sig_β, ret_β.
+    repeat (split; [assumption|]). eapply SA_Trans; eassumption.
+  - injection Hs; intros; subst.
+    do 5 eexists.
+    repeat split; try eassumption; try reflexivity.
+    apply SA_Refl. assumption.
+Qed.
+
 (* Typing of `plug P u` yields a typing of the plugged sub-term `u`   *)
 (* under the same context: evaluation contexts add no binders.        *)
 Lemma plug_typing_inv : forall P Γ u T,
@@ -164,6 +193,24 @@ Proof.
   - (* EC_perform_a *)
     apply typed_perform_inv in H. destruct H as [Tr [Ta [_ Ha]]].
     eapply IHP; exact Ha.
+Qed.
+
+Lemma handle_result_closed_from_plug_typing_for_markers :
+  forall Γ E E_tag n_beta Ts T_B T_R op_body body T,
+    eval_ctx Γ ->
+    Γ ⊢ₜ plug E (term_handle E_tag n_beta Ts T_B T_R op_body body) : T ->
+    ty_ty_closed 0 T_R /\ ty_lt_closed 0 T_R.
+Proof.
+  intros Γ E E_tag n_beta Ts T_B T_R op_body body T Hec Hty.
+  destruct (plug_typing_inv E Γ (term_handle E_tag n_beta Ts T_B T_R op_body body) T Hty)
+    as [Th Hhandle].
+  apply handle_typing_inv_for_markers in Hhandle.
+  destruct Hhandle as
+    (n_α & sig & ret & sig_β & ret_β & Heff & HlenTs & HwfTs & HwfTB & HwfTR
+     & Hnl & Hbr & Hsigβ & Hretβ & Hop & Hbody & Hsub).
+  split.
+  - eapply ty_wf_eval_ctx_ty_closed; eauto.
+  - eapply ty_wf_eval_ctx_lt_closed; eauto.
 Qed.
 
 (* ------------------------------------------------------------------ *)
@@ -357,6 +404,14 @@ Definition marker_annots_list_no_local (ts : list term) : Prop :=
   Forall (fun mt => no_local_ty (snd mt) = true)
          (List.concat (List.map marker_annots ts)).
 
+Definition marker_annots_closed (t : term) : Prop :=
+  Forall (fun mt => ty_ty_closed 0 (snd mt) /\ ty_lt_closed 0 (snd mt))
+         (marker_annots t).
+
+Definition marker_annots_list_closed (ts : list term) : Prop :=
+  Forall (fun mt => ty_ty_closed 0 (snd mt) /\ ty_lt_closed 0 (snd mt))
+         (List.concat (List.map marker_annots ts)).
+
 Definition marker_types_safe (t : term) : Prop :=
   marker_types_ok t.
 
@@ -370,6 +425,102 @@ Lemma marker_types_safe_empty : forall t,
   marker_annots t = [] -> marker_types_safe t.
 Proof.
   intros t Hann m T U Hin. rewrite Hann in Hin. inversion Hin.
+Qed.
+
+Lemma marker_annots_no_rt_cap : forall t,
+  has_rt_cap t = false -> marker_annots t = [].
+Proof.
+  apply (term_list_ind
+    (fun t => has_rt_cap t = false -> marker_annots t = [])
+    (fun ts =>
+       (fix go (ts : list term) : bool :=
+          match ts with
+          | [] => false
+          | u :: rest => orb (has_rt_cap u) (go rest)
+          end) ts = false ->
+       List.concat (List.map marker_annots ts) = [])).
+  - intros n H. reflexivity.
+  - intros t1 t2 IH1 IH2 H. simpl in *.
+    apply Bool.orb_false_iff in H as [H1 H2].
+    rewrite (IH1 H1), (IH2 H2). reflexivity.
+  - intros body T IH H. simpl in *. apply IH. exact H.
+  - intros t T IH H. simpl in *. apply IH. exact H.
+  - intros bound body IH H. simpl in *. apply IH. exact H.
+  - intros t l IH H. simpl in *. apply IH. exact H.
+  - intros body IH H. simpl in *. apply IH. exact H.
+  - intros K l lts Ts ts IH H. simpl in *. apply IH. exact H.
+  - intros scrut tag n_lt arity yes no IHs IHy IHn H. simpl in *.
+    apply Bool.orb_false_iff in H as [Hs Hyn].
+    apply Bool.orb_false_iff in Hyn as [Hy Hn].
+    rewrite (IHs Hs), (IHy Hy), (IHn Hn). reflexivity.
+  - intros E n_beta Ts T_B T_R op_body body IHop IHbody H. simpl in *.
+    apply Bool.orb_false_iff in H as [Hop Hbody].
+    rewrite (IHop Hop), (IHbody Hbody). reflexivity.
+  - intros recv Ss arg IHrecv IHarg H. simpl in *.
+    apply Bool.orb_false_iff in H as [Hr Ha].
+    rewrite (IHrecv Hr), (IHarg Ha). reflexivity.
+  - intros E m n_beta Ts T_R op_body IHop H. simpl in H. discriminate.
+  - intros m T_B T_R body IH H. simpl in H. discriminate.
+  - intros m T_B T_R body IH H. simpl in H. discriminate.
+  - intros H. reflexivity.
+  - intros t ts IHt IHts H. simpl in *.
+    apply Bool.orb_false_iff in H as [Ht Hts].
+    rewrite (IHt Ht), (IHts Hts). reflexivity.
+Qed.
+
+Lemma marker_annots_closed_no_rt_cap : forall t,
+  has_rt_cap t = false -> marker_annots_closed t.
+Proof.
+  intros t Hcap. unfold marker_annots_closed.
+  rewrite (marker_annots_no_rt_cap t Hcap). constructor.
+Qed.
+
+Lemma marker_types_safe_no_rt_cap : forall t,
+  has_rt_cap t = false -> marker_types_safe t.
+Proof.
+  intros t Hcap. apply marker_types_safe_empty.
+  apply marker_annots_no_rt_cap. exact Hcap.
+Qed.
+
+Lemma marker_ok_no_rt_cap : forall t ms,
+  has_rt_cap t = false -> marker_ok ms t.
+Proof.
+  apply (term_list_ind
+    (fun t => forall ms, has_rt_cap t = false -> marker_ok ms t)
+    (fun ts => forall ms,
+       (fix go (ts : list term) : bool :=
+          match ts with
+          | [] => false
+          | u :: rest => orb (has_rt_cap u) (go rest)
+          end) ts = false ->
+       (fix marker_ok_list (ts : list term) : Prop :=
+          match ts with
+          | [] => True
+          | u :: rest => marker_ok ms u /\ marker_ok_list rest
+          end) ts)).
+  - intros n ms H. exact I.
+  - intros t1 t2 IH1 IH2 ms H. simpl in *.
+    apply Bool.orb_false_iff in H as [H1 H2]. split; [apply IH1 | apply IH2]; assumption.
+  - intros body T IH ms H. simpl in *. apply IH. exact H.
+  - intros t T IH ms H. simpl in *. apply IH. exact H.
+  - intros bound body IH ms H. simpl in *. apply IH. exact H.
+  - intros t l IH ms H. simpl in *. apply IH. exact H.
+  - intros body IH ms H. simpl in *. apply IH. exact H.
+  - intros K l lts Ts ts IH ms H. simpl in *. apply IH. exact H.
+  - intros scrut tag n_lt arity yes no IHs IHy IHn ms H. simpl in *.
+    apply Bool.orb_false_iff in H as [Hs Hyn].
+    apply Bool.orb_false_iff in Hyn as [Hy Hn].
+    repeat split; [apply IHs | apply IHy | apply IHn]; assumption.
+  - intros E n_beta Ts T_B T_R op_body body IHop IHbody ms H. simpl in *.
+    apply Bool.orb_false_iff in H as [Hop Hbody]. split; [apply IHop | apply IHbody]; assumption.
+  - intros recv Ss arg IHrecv IHarg ms H. simpl in *.
+    apply Bool.orb_false_iff in H as [Hr Ha]. split; [apply IHrecv | apply IHarg]; assumption.
+  - intros E m n_beta Ts T_R op_body IHop ms H. simpl in H. discriminate.
+  - intros m T_B T_R body IH ms H. simpl in H. discriminate.
+  - intros m T_B T_R body IH ms H. simpl in H. discriminate.
+  - intros ms H. exact I.
+  - intros t ts IHt IHts ms H. simpl in *.
+    apply Bool.orb_false_iff in H as [Ht Hts]. split; [apply IHt | apply IHts]; assumption.
 Qed.
 
 Lemma marker_types_safe_incl : forall sub whole,
@@ -506,6 +657,173 @@ Proof.
   - intros B A IHB IHA c. simpl. rewrite IHB, IHA. reflexivity.
   - intro c. reflexivity.
   - intros A Ts IHA IHTs c. simpl. rewrite IHA, IHTs. reflexivity.
+Qed.
+
+Lemma no_local_lt_closed : forall l c,
+  no_local_lt l = true -> lt_lt_closed c l.
+Proof.
+  induction l as [x| | |l1 IH1 l2 IH2]; intros c H; simpl in *.
+  - discriminate.
+  - exact I.
+  - discriminate.
+  - apply Bool.andb_true_iff in H as [H1 H2]. split; [apply IH1 | apply IH2]; assumption.
+Qed.
+
+Lemma no_local_ty_ty_closed : forall T c,
+  no_local_ty T = true -> ty_ty_closed c T.
+Proof.
+  apply (type_list_ind
+    (fun T => forall c, no_local_ty T = true -> ty_ty_closed c T)
+    (fun Ts => forall c,
+      fold_right (fun A acc => andb (no_local_ty A) acc) true Ts = true ->
+      tys_ty_closed c Ts)).
+  - intros n c H. simpl in H. discriminate.
+  - intros A l B IHA IHB c H. simpl in *.
+    apply Bool.andb_true_iff in H as [HA Hrest].
+    apply Bool.andb_true_iff in Hrest as [_ HB].
+    split; [apply IHA | apply IHB]; assumption.
+  - intros K l Ts IHTs c H. simpl in *.
+    apply Bool.andb_true_iff in H as [_ HTs].
+    apply IHTs. exact HTs.
+  - intros A IHA c H. simpl in *. apply IHA. exact H.
+  - intros B A IHB IHA c H. simpl in *.
+    apply Bool.andb_true_iff in H as [HB HA].
+    split; [apply IHB | apply IHA]; assumption.
+  - intros c H. exact I.
+  - intros A Ts IHA IHTs c H. simpl in *.
+    apply Bool.andb_true_iff in H as [HA HTs].
+    split; [apply IHA | apply IHTs]; assumption.
+Qed.
+
+Lemma no_local_tys_ty_closed : forall Ts c,
+  fold_right (fun A acc => andb (no_local_ty A) acc) true Ts = true ->
+  tys_ty_closed c Ts.
+Proof.
+  induction Ts as [|T Ts IH]; intros c H; simpl in *.
+  - exact I.
+  - apply Bool.andb_true_iff in H as [HT HTs].
+    split; [apply no_local_ty_ty_closed | apply IH]; assumption.
+Qed.
+
+Lemma no_local_ty_lt_closed : forall T c,
+  no_local_ty T = true -> ty_lt_closed c T.
+Proof.
+  apply (type_list_ind
+    (fun T => forall c, no_local_ty T = true -> ty_lt_closed c T)
+    (fun Ts => forall c,
+      fold_right (fun A acc => andb (no_local_ty A) acc) true Ts = true ->
+      tys_lt_closed c Ts)).
+  - intros n c H. simpl in H. discriminate.
+  - intros A l B IHA IHB c H. simpl in *.
+    apply Bool.andb_true_iff in H as [HA Hrest].
+    apply Bool.andb_true_iff in Hrest as [Hl HB].
+    repeat split.
+    + apply IHA. exact HA.
+    + apply no_local_lt_closed. exact Hl.
+    + apply IHB. exact HB.
+  - intros K l Ts IHTs c H. simpl in *.
+    apply Bool.andb_true_iff in H as [Hl HTs].
+    split; [apply no_local_lt_closed | apply IHTs]; assumption.
+  - intros A IHA c H. simpl in *. apply IHA. exact H.
+  - intros B A IHB IHA c H. simpl in *.
+    apply Bool.andb_true_iff in H as [HB HA].
+    split; [apply IHB | apply IHA]; assumption.
+  - intros c H. exact I.
+  - intros A Ts IHA IHTs c H. simpl in *.
+    apply Bool.andb_true_iff in H as [HA HTs].
+    split; [apply IHA | apply IHTs]; assumption.
+Qed.
+
+Lemma no_local_tys_lt_closed : forall Ts c,
+  fold_right (fun A acc => andb (no_local_ty A) acc) true Ts = true ->
+  tys_lt_closed c Ts.
+Proof.
+  induction Ts as [|T Ts IH]; intros c H; simpl in *.
+  - exact I.
+  - apply Bool.andb_true_iff in H as [HT HTs].
+    split; [apply no_local_ty_lt_closed | apply IH]; assumption.
+Qed.
+
+Lemma shift_ty_no_local_id : forall T amount cutoff,
+  no_local_ty T = true -> shift_ty amount cutoff T = T.
+Proof.
+  intros T amount cutoff Hnl.
+  apply shift_ty_in_ty_closed. apply no_local_ty_ty_closed. exact Hnl.
+Qed.
+
+Lemma shift_lt_in_ty_no_local_id : forall T amount cutoff,
+  no_local_ty T = true -> shift_lt_in_ty amount cutoff T = T.
+Proof.
+  intros T amount cutoff Hnl.
+  apply shift_lt_in_type_closed. apply no_local_ty_lt_closed. exact Hnl.
+Qed.
+
+Lemma subst_ty_no_local_id : forall T var R,
+  no_local_ty T = true -> subst_ty var R T = T.
+Proof.
+  intros T var R Hnl.
+  apply subst_ty_ty_closed_id with (c := 0); [apply no_local_ty_ty_closed; exact Hnl | lia].
+Qed.
+
+Lemma subst_lt_in_ty_no_local_id : forall T var R,
+  no_local_ty T = true -> subst_lt_in_ty var R T = T.
+Proof.
+  intros T var R Hnl.
+  apply subst_lt_in_type_closed with (c := var).
+  apply no_local_ty_lt_closed. exact Hnl.
+Qed.
+
+Lemma shift_ty_closed0_id : forall T amount cutoff,
+  ty_ty_closed 0 T -> shift_ty amount cutoff T = T.
+Proof.
+  intros T amount cutoff Hclosed.
+  apply shift_ty_in_ty_closed with (c := cutoff).
+  eapply ty_ty_closed_mono; [apply Nat.le_0_l | exact Hclosed].
+Qed.
+
+Lemma shift_lt_in_ty_closed0_id : forall T amount cutoff,
+  ty_lt_closed 0 T -> shift_lt_in_ty amount cutoff T = T.
+Proof.
+  intros T amount cutoff Hclosed.
+  apply shift_lt_in_type_closed with (c := cutoff).
+  eapply ty_lt_closed_mono; [apply Nat.le_0_l | exact Hclosed].
+Qed.
+
+Lemma subst_ty_closed0_id : forall T var R,
+  ty_ty_closed 0 T -> subst_ty var R T = T.
+Proof.
+  intros T var R Hclosed.
+  apply subst_ty_ty_closed_id with (c := 0); [exact Hclosed | lia].
+Qed.
+
+Lemma subst_lt_in_ty_closed0_id : forall T var R,
+  ty_lt_closed 0 T -> subst_lt_in_ty var R T = T.
+Proof.
+  intros T var R Hclosed.
+  apply subst_lt_in_type_closed with (c := var).
+  eapply ty_lt_closed_mono; [apply Nat.le_0_l | exact Hclosed].
+Qed.
+
+Lemma marker_annots_no_local_closed : forall t,
+  marker_annots_no_local t -> marker_annots_closed t.
+Proof.
+  intros t Hnl.
+  unfold marker_annots_no_local, marker_annots_closed in *.
+  eapply Forall_impl; [|exact Hnl].
+  intros [m T] HT. simpl in *. split.
+  - apply no_local_ty_ty_closed. exact HT.
+  - apply no_local_ty_lt_closed. exact HT.
+Qed.
+
+Lemma marker_annots_list_no_local_closed : forall ts,
+  marker_annots_list_no_local ts -> marker_annots_list_closed ts.
+Proof.
+  intros ts Hnl.
+  unfold marker_annots_list_no_local, marker_annots_list_closed in *.
+  eapply Forall_impl; [|exact Hnl].
+  intros [m T] HT. simpl in *. split.
+  - apply no_local_ty_ty_closed. exact HT.
+  - apply no_local_ty_lt_closed. exact HT.
 Qed.
 
 Lemma marker_annots_no_local_shift_tm : forall t amount cutoff,
@@ -906,6 +1224,1573 @@ Proof.
   - apply IH. apply marker_annots_no_local_subst_ty_in_tm. exact Ht.
 Qed.
 
+(* go_eq_map for subst_ty_in_tm (the other go_eq_map lemmas live upstream). *)
+Lemma subst_ty_in_tm_go_eq_map : forall var R ts,
+  (fix go ts := match ts with [] => [] | u :: rest => subst_ty_in_tm var R u :: go rest end) ts =
+  List.map (subst_ty_in_tm var R) ts.
+Proof. intros; induction ts; simpl; congruence. Qed.
+
+Lemma marker_annots_shift_tm : forall t amount cutoff,
+  marker_annots (shift_tm amount cutoff t) = marker_annots t.
+Proof.
+  apply (term_list_ind
+    (fun t => forall amount cutoff,
+       marker_annots (shift_tm amount cutoff t) = marker_annots t)
+    (fun ts => forall amount cutoff,
+       List.concat (List.map marker_annots (List.map (shift_tm amount cutoff) ts)) =
+       List.concat (List.map marker_annots ts))).
+  - intros n amount cutoff. reflexivity.
+  - intros t1 t2 IH1 IH2 amount cutoff. simpl.
+    rewrite IH1, IH2. reflexivity.
+  - intros body T IH amount cutoff. simpl. apply IH.
+  - intros t T IH amount cutoff. simpl. apply IH.
+  - intros bound body IH amount cutoff. simpl. apply IH.
+  - intros t l IH amount cutoff. simpl. apply IH.
+  - intros body IH amount cutoff. simpl. apply IH.
+  - intros K l lts Ts ts IH amount cutoff. simpl.
+    rewrite shift_tm_go_eq_map. apply IH.
+  - intros scrut tag n_lt arity yes no IHs IHy IHn amount cutoff. simpl.
+    rewrite IHs, IHy, IHn. reflexivity.
+  - intros E n_beta Ts T_B T_R op_body body IHop IHbody amount cutoff. simpl.
+    rewrite IHop, IHbody. reflexivity.
+  - intros recv Ss arg IHrecv IHarg amount cutoff. simpl.
+    rewrite IHrecv, IHarg. reflexivity.
+  - intros E m n_beta Ts T_R op_body IHop amount cutoff. simpl.
+    rewrite IHop. reflexivity.
+  - intros m T_B T_R t IH amount cutoff. simpl.
+    rewrite IH. reflexivity.
+  - intros m T_B T_R b IH amount cutoff. simpl.
+    rewrite IH. reflexivity.
+  - intros amount cutoff. reflexivity.
+  - intros t ts IHt IHts amount cutoff. simpl.
+    rewrite IHt, IHts. reflexivity.
+Qed.
+
+Lemma marker_annots_list_shift_tm : forall ts amount cutoff,
+  List.concat (List.map marker_annots (List.map (shift_tm amount cutoff) ts)) =
+  List.concat (List.map marker_annots ts).
+Proof.
+  induction ts as [|t ts IH]; intros amount cutoff; simpl.
+  - reflexivity.
+  - rewrite marker_annots_shift_tm, IH. reflexivity.
+Qed.
+
+Lemma marker_annots_shift_ectx_tm : forall E hole amount cutoff,
+  marker_annots (plug (shift_ectx_tm amount cutoff E) hole) = marker_annots (plug E hole).
+Proof.
+  induction E; intros hole amount cutoff; simpl.
+  - reflexivity.
+  - rewrite IHE, marker_annots_shift_tm. reflexivity.
+  - rewrite marker_annots_shift_tm, IHE. reflexivity.
+  - apply IHE.
+  - apply IHE.
+  - repeat rewrite List.map_app. repeat rewrite List.concat_app. simpl.
+    rewrite marker_annots_list_shift_tm, IHE, marker_annots_list_shift_tm. reflexivity.
+  - rewrite IHE, !marker_annots_shift_tm. reflexivity.
+  - rewrite IHE. reflexivity.
+  - rewrite IHE, marker_annots_shift_tm. reflexivity.
+  - rewrite marker_annots_shift_tm, IHE. reflexivity.
+Qed.
+
+Lemma marker_annots_shift_ty_in_tm_no_local : forall t amount cutoff,
+  marker_annots_no_local t ->
+  marker_annots (shift_ty_in_tm amount cutoff t) = marker_annots t.
+Proof.
+  apply (term_list_ind
+    (fun t => forall amount cutoff,
+       marker_annots_no_local t ->
+       marker_annots (shift_ty_in_tm amount cutoff t) = marker_annots t)
+    (fun ts => forall amount cutoff,
+       marker_annots_list_no_local ts ->
+       List.concat (List.map marker_annots (List.map (shift_ty_in_tm amount cutoff) ts)) =
+       List.concat (List.map marker_annots ts))).
+  - intros n amount cutoff H. reflexivity.
+  - intros t1 t2 IH1 IH2 amount cutoff H. unfold marker_annots_no_local in *.
+    simpl in *. apply Forall_app in H as [H1 H2].
+    rewrite (IH1 amount cutoff H1), (IH2 amount cutoff H2). reflexivity.
+  - intros body T IH amount cutoff H. simpl in *. apply IH. exact H.
+  - intros t T IH amount cutoff H. simpl in *. apply IH. exact H.
+  - intros bound body IH amount cutoff H. simpl in *. apply IH. exact H.
+  - intros t l IH amount cutoff H. simpl in *. apply IH. exact H.
+  - intros body IH amount cutoff H. simpl in *. apply IH. exact H.
+  - intros K l lts Ts ts IH amount cutoff H. simpl in *.
+    rewrite shift_ty_in_tm_go_eq_map.
+    unfold marker_annots_no_local in H. fold marker_annots_list_no_local in H.
+    apply IH. exact H.
+  - intros scrut tag n_lt arity yes no IHs IHy IHn amount cutoff H.
+    unfold marker_annots_no_local in *. simpl in *.
+    repeat rewrite Forall_app in H. destruct H as [Hs [Hy Hn]].
+    rewrite (IHs amount cutoff Hs), (IHy amount cutoff Hy), (IHn amount cutoff Hn).
+    reflexivity.
+  - intros E n_beta Ts T_B T_R op_body body IHop IHbody amount cutoff H.
+    unfold marker_annots_no_local in *. simpl in *.
+    apply Forall_app in H as [Hop Hbody].
+    rewrite (IHop amount (cutoff + n_beta) Hop), (IHbody amount cutoff Hbody).
+    reflexivity.
+  - intros recv Ss arg IHrecv IHarg amount cutoff H.
+    unfold marker_annots_no_local in *. simpl in *.
+    apply Forall_app in H as [Hr Ha].
+    rewrite (IHrecv amount cutoff Hr), (IHarg amount cutoff Ha). reflexivity.
+  - intros E m n_beta Ts T_R op_body IHop amount cutoff H.
+    unfold marker_annots_no_local in *. simpl in *.
+    inversion H as [|mt rest Hhead Htail]; subst.
+    rewrite (shift_ty_no_local_id T_R amount cutoff Hhead).
+    rewrite (IHop amount (cutoff + n_beta) Htail). reflexivity.
+  - intros m T_B T_R t IH amount cutoff H.
+    unfold marker_annots_no_local in *. simpl in *.
+    inversion H as [|mt rest Hhead Htail]; subst.
+    rewrite (shift_ty_no_local_id T_R amount cutoff Hhead).
+    rewrite (IH amount cutoff Htail). reflexivity.
+  - intros m T_B T_R b IH amount cutoff H.
+    unfold marker_annots_no_local in *. simpl in *.
+    inversion H as [|mt rest Hhead Htail]; subst.
+    rewrite (shift_ty_no_local_id T_R amount cutoff Hhead).
+    rewrite (IH amount cutoff Htail). reflexivity.
+  - intros amount cutoff H. reflexivity.
+  - intros t ts IHt IHts amount cutoff H.
+    unfold marker_annots_list_no_local in *. simpl in *.
+    apply Forall_app in H as [Ht Hts].
+    rewrite (IHt amount cutoff Ht), (IHts amount cutoff Hts). reflexivity.
+Qed.
+
+Lemma marker_annots_shift_lt_in_tm_no_local : forall t amount cutoff,
+  marker_annots_no_local t ->
+  marker_annots (shift_lt_in_tm amount cutoff t) = marker_annots t.
+Proof.
+  apply (term_list_ind
+    (fun t => forall amount cutoff,
+       marker_annots_no_local t ->
+       marker_annots (shift_lt_in_tm amount cutoff t) = marker_annots t)
+    (fun ts => forall amount cutoff,
+       marker_annots_list_no_local ts ->
+       List.concat (List.map marker_annots (List.map (shift_lt_in_tm amount cutoff) ts)) =
+       List.concat (List.map marker_annots ts))).
+  - intros n amount cutoff H. reflexivity.
+  - intros t1 t2 IH1 IH2 amount cutoff H. unfold marker_annots_no_local in *.
+    simpl in *. apply Forall_app in H as [H1 H2].
+    rewrite (IH1 amount cutoff H1), (IH2 amount cutoff H2). reflexivity.
+  - intros body T IH amount cutoff H. simpl in *. apply IH. exact H.
+  - intros t T IH amount cutoff H. simpl in *. apply IH. exact H.
+  - intros bound body IH amount cutoff H. simpl in *. apply IH. exact H.
+  - intros t l IH amount cutoff H. simpl in *. apply IH. exact H.
+  - intros body IH amount cutoff H. simpl in *. apply IH. exact H.
+  - intros K l lts Ts ts IH amount cutoff H. simpl in *.
+    rewrite shift_lt_in_tm_go_eq_map.
+    unfold marker_annots_no_local in H. fold marker_annots_list_no_local in H.
+    apply IH. exact H.
+  - intros scrut tag n_lt arity yes no IHs IHy IHn amount cutoff H.
+    unfold marker_annots_no_local in *. simpl in *.
+    repeat rewrite Forall_app in H. destruct H as [Hs [Hy Hn]].
+    rewrite (IHs amount cutoff Hs), (IHy amount (cutoff + n_lt) Hy), (IHn amount cutoff Hn).
+    reflexivity.
+  - intros E n_beta Ts T_B T_R op_body body IHop IHbody amount cutoff H.
+    unfold marker_annots_no_local in *. simpl in *.
+    apply Forall_app in H as [Hop Hbody].
+    rewrite (IHop amount cutoff Hop), (IHbody amount cutoff Hbody). reflexivity.
+  - intros recv Ss arg IHrecv IHarg amount cutoff H.
+    unfold marker_annots_no_local in *. simpl in *.
+    apply Forall_app in H as [Hr Ha].
+    rewrite (IHrecv amount cutoff Hr), (IHarg amount cutoff Ha). reflexivity.
+  - intros E m n_beta Ts T_R op_body IHop amount cutoff H.
+    unfold marker_annots_no_local in *. simpl in *.
+    inversion H as [|mt rest Hhead Htail]; subst.
+    rewrite (shift_lt_in_ty_no_local_id T_R amount cutoff Hhead).
+    rewrite (IHop amount cutoff Htail). reflexivity.
+  - intros m T_B T_R t IH amount cutoff H.
+    unfold marker_annots_no_local in *. simpl in *.
+    inversion H as [|mt rest Hhead Htail]; subst.
+    rewrite (shift_lt_in_ty_no_local_id T_R amount cutoff Hhead).
+    rewrite (IH amount cutoff Htail). reflexivity.
+  - intros m T_B T_R b IH amount cutoff H.
+    unfold marker_annots_no_local in *. simpl in *.
+    inversion H as [|mt rest Hhead Htail]; subst.
+    rewrite (shift_lt_in_ty_no_local_id T_R amount cutoff Hhead).
+    rewrite (IH amount cutoff Htail). reflexivity.
+  - intros amount cutoff H. reflexivity.
+  - intros t ts IHt IHts amount cutoff H.
+    unfold marker_annots_list_no_local in *. simpl in *.
+    apply Forall_app in H as [Ht Hts].
+    rewrite (IHt amount cutoff Ht), (IHts amount cutoff Hts). reflexivity.
+Qed.
+
+Lemma marker_annots_shift_ty_in_tm_closed : forall t amount cutoff,
+  marker_annots_closed t ->
+  marker_annots (shift_ty_in_tm amount cutoff t) = marker_annots t.
+Proof.
+  apply (term_list_ind
+    (fun t => forall amount cutoff,
+       marker_annots_closed t ->
+       marker_annots (shift_ty_in_tm amount cutoff t) = marker_annots t)
+    (fun ts => forall amount cutoff,
+       marker_annots_list_closed ts ->
+       List.concat (List.map marker_annots (List.map (shift_ty_in_tm amount cutoff) ts)) =
+       List.concat (List.map marker_annots ts))).
+  - intros n amount cutoff H. reflexivity.
+  - intros t1 t2 IH1 IH2 amount cutoff H. unfold marker_annots_closed in *.
+    simpl in *. apply Forall_app in H as [H1 H2].
+    rewrite (IH1 amount cutoff H1), (IH2 amount cutoff H2). reflexivity.
+  - intros body T IH amount cutoff H. simpl in *. apply IH. exact H.
+  - intros t T IH amount cutoff H. simpl in *. apply IH. exact H.
+  - intros bound body IH amount cutoff H. simpl in *. apply IH. exact H.
+  - intros t l IH amount cutoff H. simpl in *. apply IH. exact H.
+  - intros body IH amount cutoff H. simpl in *. apply IH. exact H.
+  - intros K l lts Ts ts IH amount cutoff H. simpl in *.
+    rewrite shift_ty_in_tm_go_eq_map.
+    unfold marker_annots_closed in H. fold marker_annots_list_closed in H.
+    apply IH. exact H.
+  - intros scrut tag n_lt arity yes no IHs IHy IHn amount cutoff H.
+    unfold marker_annots_closed in *. simpl in *.
+    repeat rewrite Forall_app in H. destruct H as [Hs [Hy Hn]].
+    rewrite (IHs amount cutoff Hs), (IHy amount cutoff Hy), (IHn amount cutoff Hn).
+    reflexivity.
+  - intros E n_beta Ts T_B T_R op_body body IHop IHbody amount cutoff H.
+    unfold marker_annots_closed in *. simpl in *.
+    apply Forall_app in H as [Hop Hbody].
+    rewrite (IHop amount (cutoff + n_beta) Hop), (IHbody amount cutoff Hbody).
+    reflexivity.
+  - intros recv Ss arg IHrecv IHarg amount cutoff H.
+    unfold marker_annots_closed in *. simpl in *.
+    apply Forall_app in H as [Hr Ha].
+    rewrite (IHrecv amount cutoff Hr), (IHarg amount cutoff Ha). reflexivity.
+  - intros E m n_beta Ts T_R op_body IHop amount cutoff H.
+    unfold marker_annots_closed in *. simpl in *.
+    inversion H as [|mt rest Hhead Htail]; subst.
+    destruct Hhead as [HTy _].
+    rewrite (shift_ty_closed0_id T_R amount cutoff HTy).
+    rewrite (IHop amount (cutoff + n_beta) Htail). reflexivity.
+  - intros m T_B T_R t IH amount cutoff H.
+    unfold marker_annots_closed in *. simpl in *.
+    inversion H as [|mt rest Hhead Htail]; subst.
+    destruct Hhead as [HTy _].
+    rewrite (shift_ty_closed0_id T_R amount cutoff HTy).
+    rewrite (IH amount cutoff Htail). reflexivity.
+  - intros m T_B T_R b IH amount cutoff H.
+    unfold marker_annots_closed in *. simpl in *.
+    inversion H as [|mt rest Hhead Htail]; subst.
+    destruct Hhead as [HTy _].
+    rewrite (shift_ty_closed0_id T_R amount cutoff HTy).
+    rewrite (IH amount cutoff Htail). reflexivity.
+  - intros amount cutoff H. reflexivity.
+  - intros t ts IHt IHts amount cutoff H.
+    unfold marker_annots_list_closed in *. simpl in *.
+    apply Forall_app in H as [Ht Hts].
+    rewrite (IHt amount cutoff Ht), (IHts amount cutoff Hts). reflexivity.
+Qed.
+
+Lemma marker_annots_shift_lt_in_tm_closed : forall t amount cutoff,
+  marker_annots_closed t ->
+  marker_annots (shift_lt_in_tm amount cutoff t) = marker_annots t.
+Proof.
+  apply (term_list_ind
+    (fun t => forall amount cutoff,
+       marker_annots_closed t ->
+       marker_annots (shift_lt_in_tm amount cutoff t) = marker_annots t)
+    (fun ts => forall amount cutoff,
+       marker_annots_list_closed ts ->
+       List.concat (List.map marker_annots (List.map (shift_lt_in_tm amount cutoff) ts)) =
+       List.concat (List.map marker_annots ts))).
+  - intros n amount cutoff H. reflexivity.
+  - intros t1 t2 IH1 IH2 amount cutoff H. unfold marker_annots_closed in *.
+    simpl in *. apply Forall_app in H as [H1 H2].
+    rewrite (IH1 amount cutoff H1), (IH2 amount cutoff H2). reflexivity.
+  - intros body T IH amount cutoff H. simpl in *. apply IH. exact H.
+  - intros t T IH amount cutoff H. simpl in *. apply IH. exact H.
+  - intros bound body IH amount cutoff H. simpl in *. apply IH. exact H.
+  - intros t l IH amount cutoff H. simpl in *. apply IH. exact H.
+  - intros body IH amount cutoff H. simpl in *. apply IH. exact H.
+  - intros K l lts Ts ts IH amount cutoff H. simpl in *.
+    rewrite shift_lt_in_tm_go_eq_map.
+    unfold marker_annots_closed in H. fold marker_annots_list_closed in H.
+    apply IH. exact H.
+  - intros scrut tag n_lt arity yes no IHs IHy IHn amount cutoff H.
+    unfold marker_annots_closed in *. simpl in *.
+    repeat rewrite Forall_app in H. destruct H as [Hs [Hy Hn]].
+    rewrite (IHs amount cutoff Hs), (IHy amount (cutoff + n_lt) Hy), (IHn amount cutoff Hn).
+    reflexivity.
+  - intros E n_beta Ts T_B T_R op_body body IHop IHbody amount cutoff H.
+    unfold marker_annots_closed in *. simpl in *.
+    apply Forall_app in H as [Hop Hbody].
+    rewrite (IHop amount cutoff Hop), (IHbody amount cutoff Hbody). reflexivity.
+  - intros recv Ss arg IHrecv IHarg amount cutoff H.
+    unfold marker_annots_closed in *. simpl in *.
+    apply Forall_app in H as [Hr Ha].
+    rewrite (IHrecv amount cutoff Hr), (IHarg amount cutoff Ha). reflexivity.
+  - intros E m n_beta Ts T_R op_body IHop amount cutoff H.
+    unfold marker_annots_closed in *. simpl in *.
+    inversion H as [|mt rest Hhead Htail]; subst.
+    destruct Hhead as [_ HLt].
+    rewrite (shift_lt_in_ty_closed0_id T_R amount cutoff HLt).
+    rewrite (IHop amount cutoff Htail). reflexivity.
+  - intros m T_B T_R t IH amount cutoff H.
+    unfold marker_annots_closed in *. simpl in *.
+    inversion H as [|mt rest Hhead Htail]; subst.
+    destruct Hhead as [_ HLt].
+    rewrite (shift_lt_in_ty_closed0_id T_R amount cutoff HLt).
+    rewrite (IH amount cutoff Htail). reflexivity.
+  - intros m T_B T_R b IH amount cutoff H.
+    unfold marker_annots_closed in *. simpl in *.
+    inversion H as [|mt rest Hhead Htail]; subst.
+    destruct Hhead as [_ HLt].
+    rewrite (shift_lt_in_ty_closed0_id T_R amount cutoff HLt).
+    rewrite (IH amount cutoff Htail). reflexivity.
+  - intros amount cutoff H. reflexivity.
+  - intros t ts IHt IHts amount cutoff H.
+    unfold marker_annots_list_closed in *. simpl in *.
+    apply Forall_app in H as [Ht Hts].
+    rewrite (IHt amount cutoff Ht), (IHts amount cutoff Hts). reflexivity.
+Qed.
+
+Lemma marker_annots_closed_shift_tm : forall t amount cutoff,
+  marker_annots_closed t -> marker_annots_closed (shift_tm amount cutoff t).
+Proof.
+  intros t amount cutoff H.
+  unfold marker_annots_closed in *. rewrite marker_annots_shift_tm. exact H.
+Qed.
+
+Lemma marker_annots_closed_shift_ty_in_tm : forall t amount cutoff,
+  marker_annots_closed t -> marker_annots_closed (shift_ty_in_tm amount cutoff t).
+Proof.
+  intros t amount cutoff H.
+  unfold marker_annots_closed in *. rewrite marker_annots_shift_ty_in_tm_closed by exact H. exact H.
+Qed.
+
+Lemma marker_annots_closed_shift_lt_in_tm : forall t amount cutoff,
+  marker_annots_closed t -> marker_annots_closed (shift_lt_in_tm amount cutoff t).
+Proof.
+  intros t amount cutoff H.
+  unfold marker_annots_closed in *. rewrite marker_annots_shift_lt_in_tm_closed by exact H. exact H.
+Qed.
+
+Lemma marker_annots_subst_ty_in_tm_no_local : forall t var replacement,
+  marker_annots_no_local t ->
+  marker_annots (subst_ty_in_tm var replacement t) = marker_annots t.
+Proof.
+  apply (term_list_ind
+    (fun t => forall var replacement,
+       marker_annots_no_local t ->
+       marker_annots (subst_ty_in_tm var replacement t) = marker_annots t)
+    (fun ts => forall var replacement,
+       marker_annots_list_no_local ts ->
+       List.concat (List.map marker_annots (List.map (subst_ty_in_tm var replacement) ts)) =
+       List.concat (List.map marker_annots ts))).
+  - intros n var replacement H. reflexivity.
+  - intros t1 t2 IH1 IH2 var replacement H. unfold marker_annots_no_local in *.
+    simpl in *. apply Forall_app in H as [H1 H2].
+    rewrite (IH1 var replacement H1), (IH2 var replacement H2). reflexivity.
+  - intros body T IH var replacement H. simpl in *. apply IH. exact H.
+  - intros t T IH var replacement H. simpl in *. apply IH. exact H.
+  - intros bound body IH var replacement H. simpl in *. apply IH. exact H.
+  - intros t l IH var replacement H. simpl in *. apply IH. exact H.
+  - intros body IH var replacement H. simpl in *. apply IH. exact H.
+  - intros K l lts Ts ts IH var replacement H. simpl in *.
+    rewrite subst_ty_in_tm_go_eq_map.
+    unfold marker_annots_no_local in H. fold marker_annots_list_no_local in H.
+    apply IH. exact H.
+  - intros scrut tag n_lt arity yes no IHs IHy IHn var replacement H.
+    unfold marker_annots_no_local in *. simpl in *.
+    repeat rewrite Forall_app in H. destruct H as [Hs [Hy Hn]].
+    rewrite (IHs var replacement Hs).
+    rewrite (IHy var (shift_lt_in_ty n_lt 0 replacement) Hy).
+    rewrite (IHn var replacement Hn). reflexivity.
+  - intros E n_beta Ts T_B T_R op_body body IHop IHbody var replacement H.
+    unfold marker_annots_no_local in *. simpl in *.
+    apply Forall_app in H as [Hop Hbody].
+    rewrite (IHop (var + n_beta) (shift_ty n_beta 0 replacement) Hop).
+    rewrite (IHbody var replacement Hbody). reflexivity.
+  - intros recv Ss arg IHrecv IHarg var replacement H.
+    unfold marker_annots_no_local in *. simpl in *.
+    apply Forall_app in H as [Hr Ha].
+    rewrite (IHrecv var replacement Hr), (IHarg var replacement Ha). reflexivity.
+  - intros E m n_beta Ts T_R op_body IHop var replacement H.
+    unfold marker_annots_no_local in *. simpl in *.
+    inversion H as [|mt rest Hhead Htail]; subst.
+    rewrite (subst_ty_no_local_id T_R var replacement Hhead).
+    rewrite (IHop (var + n_beta) (shift_ty n_beta 0 replacement) Htail). reflexivity.
+  - intros m T_B T_R t IH var replacement H.
+    unfold marker_annots_no_local in *. simpl in *.
+    inversion H as [|mt rest Hhead Htail]; subst.
+    rewrite (subst_ty_no_local_id T_R var replacement Hhead).
+    rewrite (IH var replacement Htail). reflexivity.
+  - intros m T_B T_R b IH var replacement H.
+    unfold marker_annots_no_local in *. simpl in *.
+    inversion H as [|mt rest Hhead Htail]; subst.
+    rewrite (subst_ty_no_local_id T_R var replacement Hhead).
+    rewrite (IH var replacement Htail). reflexivity.
+  - intros var replacement H. reflexivity.
+  - intros t ts IHt IHts var replacement H.
+    unfold marker_annots_list_no_local in *. simpl in *.
+    apply Forall_app in H as [Ht Hts].
+    rewrite (IHt var replacement Ht), (IHts var replacement Hts). reflexivity.
+Qed.
+
+Lemma marker_annots_subst_lt_in_tm_no_local : forall t var replacement,
+  marker_annots_no_local t ->
+  marker_annots (subst_lt_in_tm var replacement t) = marker_annots t.
+Proof.
+  apply (term_list_ind
+    (fun t => forall var replacement,
+       marker_annots_no_local t ->
+       marker_annots (subst_lt_in_tm var replacement t) = marker_annots t)
+    (fun ts => forall var replacement,
+       marker_annots_list_no_local ts ->
+       List.concat (List.map marker_annots (List.map (subst_lt_in_tm var replacement) ts)) =
+       List.concat (List.map marker_annots ts))).
+  - intros n var replacement H. reflexivity.
+  - intros t1 t2 IH1 IH2 var replacement H. unfold marker_annots_no_local in *.
+    simpl in *. apply Forall_app in H as [H1 H2].
+    rewrite (IH1 var replacement H1), (IH2 var replacement H2). reflexivity.
+  - intros body T IH var replacement H. simpl in *. apply IH. exact H.
+  - intros t T IH var replacement H. simpl in *. apply IH. exact H.
+  - intros bound body IH var replacement H. simpl in *. apply IH. exact H.
+  - intros t l IH var replacement H. simpl in *. apply IH. exact H.
+  - intros body IH var replacement H. simpl in *. apply IH. exact H.
+  - intros K l lts Ts ts IH var replacement H. simpl in *.
+    rewrite subst_lt_in_tm_go_eq_map.
+    unfold marker_annots_no_local in H. fold marker_annots_list_no_local in H.
+    apply IH. exact H.
+  - intros scrut tag n_lt arity yes no IHs IHy IHn var replacement H.
+    unfold marker_annots_no_local in *. simpl in *.
+    repeat rewrite Forall_app in H. destruct H as [Hs [Hy Hn]].
+    rewrite (IHs var replacement Hs).
+    rewrite (IHy (n_lt + var) (shift_lt n_lt 0 replacement) Hy).
+    rewrite (IHn var replacement Hn). reflexivity.
+  - intros E n_beta Ts T_B T_R op_body body IHop IHbody var replacement H.
+    unfold marker_annots_no_local in *. simpl in *.
+    apply Forall_app in H as [Hop Hbody].
+    rewrite (IHop var replacement Hop), (IHbody var replacement Hbody). reflexivity.
+  - intros recv Ss arg IHrecv IHarg var replacement H.
+    unfold marker_annots_no_local in *. simpl in *.
+    apply Forall_app in H as [Hr Ha].
+    rewrite (IHrecv var replacement Hr), (IHarg var replacement Ha). reflexivity.
+  - intros E m n_beta Ts T_R op_body IHop var replacement H.
+    unfold marker_annots_no_local in *. simpl in *.
+    inversion H as [|mt rest Hhead Htail]; subst.
+    rewrite (subst_lt_in_ty_no_local_id T_R var replacement Hhead).
+    rewrite (IHop var replacement Htail). reflexivity.
+  - intros m T_B T_R t IH var replacement H.
+    unfold marker_annots_no_local in *. simpl in *.
+    inversion H as [|mt rest Hhead Htail]; subst.
+    rewrite (subst_lt_in_ty_no_local_id T_R var replacement Hhead).
+    rewrite (IH var replacement Htail). reflexivity.
+  - intros m T_B T_R b IH var replacement H.
+    unfold marker_annots_no_local in *. simpl in *.
+    inversion H as [|mt rest Hhead Htail]; subst.
+    rewrite (subst_lt_in_ty_no_local_id T_R var replacement Hhead).
+    rewrite (IH var replacement Htail). reflexivity.
+  - intros var replacement H. reflexivity.
+  - intros t ts IHt IHts var replacement H.
+    unfold marker_annots_list_no_local in *. simpl in *.
+    apply Forall_app in H as [Ht Hts].
+    rewrite (IHt var replacement Ht), (IHts var replacement Hts). reflexivity.
+Qed.
+
+Lemma marker_annots_subst_ty_in_tm_closed : forall t var replacement,
+  marker_annots_closed t ->
+  marker_annots (subst_ty_in_tm var replacement t) = marker_annots t.
+Proof.
+  apply (term_list_ind
+    (fun t => forall var replacement,
+       marker_annots_closed t ->
+       marker_annots (subst_ty_in_tm var replacement t) = marker_annots t)
+    (fun ts => forall var replacement,
+       marker_annots_list_closed ts ->
+       List.concat (List.map marker_annots (List.map (subst_ty_in_tm var replacement) ts)) =
+       List.concat (List.map marker_annots ts))).
+  - intros n var replacement H. reflexivity.
+  - intros t1 t2 IH1 IH2 var replacement H. unfold marker_annots_closed in *.
+    simpl in *. apply Forall_app in H as [H1 H2].
+    rewrite (IH1 var replacement H1), (IH2 var replacement H2). reflexivity.
+  - intros body T IH var replacement H. simpl in *. apply IH. exact H.
+  - intros t T IH var replacement H. simpl in *. apply IH. exact H.
+  - intros bound body IH var replacement H. simpl in *. apply IH. exact H.
+  - intros t l IH var replacement H. simpl in *. apply IH. exact H.
+  - intros body IH var replacement H. simpl in *. apply IH. exact H.
+  - intros K l lts Ts ts IH var replacement H. simpl in *.
+    rewrite subst_ty_in_tm_go_eq_map.
+    unfold marker_annots_closed in H. fold marker_annots_list_closed in H.
+    apply IH. exact H.
+  - intros scrut tag n_lt arity yes no IHs IHy IHn var replacement H.
+    unfold marker_annots_closed in *. simpl in *.
+    repeat rewrite Forall_app in H. destruct H as [Hs [Hy Hn]].
+    rewrite (IHs var replacement Hs).
+    rewrite (IHy var (shift_lt_in_ty n_lt 0 replacement) Hy).
+    rewrite (IHn var replacement Hn). reflexivity.
+  - intros E n_beta Ts T_B T_R op_body body IHop IHbody var replacement H.
+    unfold marker_annots_closed in *. simpl in *.
+    apply Forall_app in H as [Hop Hbody].
+    rewrite (IHop (var + n_beta) (shift_ty n_beta 0 replacement) Hop).
+    rewrite (IHbody var replacement Hbody). reflexivity.
+  - intros recv Ss arg IHrecv IHarg var replacement H.
+    unfold marker_annots_closed in *. simpl in *.
+    apply Forall_app in H as [Hr Ha].
+    rewrite (IHrecv var replacement Hr), (IHarg var replacement Ha). reflexivity.
+  - intros E m n_beta Ts T_R op_body IHop var replacement H.
+    unfold marker_annots_closed in *. simpl in *.
+    inversion H as [|mt rest Hhead Htail]; subst.
+    destruct Hhead as [HTy _].
+    rewrite (subst_ty_closed0_id T_R var replacement HTy).
+    rewrite (IHop (var + n_beta) (shift_ty n_beta 0 replacement) Htail). reflexivity.
+  - intros m T_B T_R t IH var replacement H.
+    unfold marker_annots_closed in *. simpl in *.
+    inversion H as [|mt rest Hhead Htail]; subst.
+    destruct Hhead as [HTy _].
+    rewrite (subst_ty_closed0_id T_R var replacement HTy).
+    rewrite (IH var replacement Htail). reflexivity.
+  - intros m T_B T_R b IH var replacement H.
+    unfold marker_annots_closed in *. simpl in *.
+    inversion H as [|mt rest Hhead Htail]; subst.
+    destruct Hhead as [HTy _].
+    rewrite (subst_ty_closed0_id T_R var replacement HTy).
+    rewrite (IH var replacement Htail). reflexivity.
+  - intros var replacement H. reflexivity.
+  - intros t ts IHt IHts var replacement H.
+    unfold marker_annots_list_closed in *. simpl in *.
+    apply Forall_app in H as [Ht Hts].
+    rewrite (IHt var replacement Ht), (IHts var replacement Hts). reflexivity.
+Qed.
+
+Lemma marker_annots_subst_lt_in_tm_closed : forall t var replacement,
+  marker_annots_closed t ->
+  marker_annots (subst_lt_in_tm var replacement t) = marker_annots t.
+Proof.
+  apply (term_list_ind
+    (fun t => forall var replacement,
+       marker_annots_closed t ->
+       marker_annots (subst_lt_in_tm var replacement t) = marker_annots t)
+    (fun ts => forall var replacement,
+       marker_annots_list_closed ts ->
+       List.concat (List.map marker_annots (List.map (subst_lt_in_tm var replacement) ts)) =
+       List.concat (List.map marker_annots ts))).
+  - intros n var replacement H. reflexivity.
+  - intros t1 t2 IH1 IH2 var replacement H. unfold marker_annots_closed in *.
+    simpl in *. apply Forall_app in H as [H1 H2].
+    rewrite (IH1 var replacement H1), (IH2 var replacement H2). reflexivity.
+  - intros body T IH var replacement H. simpl in *. apply IH. exact H.
+  - intros t T IH var replacement H. simpl in *. apply IH. exact H.
+  - intros bound body IH var replacement H. simpl in *. apply IH. exact H.
+  - intros t l IH var replacement H. simpl in *. apply IH. exact H.
+  - intros body IH var replacement H. simpl in *. apply IH. exact H.
+  - intros K l lts Ts ts IH var replacement H. simpl in *.
+    rewrite subst_lt_in_tm_go_eq_map.
+    unfold marker_annots_closed in H. fold marker_annots_list_closed in H.
+    apply IH. exact H.
+  - intros scrut tag n_lt arity yes no IHs IHy IHn var replacement H.
+    unfold marker_annots_closed in *. simpl in *.
+    repeat rewrite Forall_app in H. destruct H as [Hs [Hy Hn]].
+    rewrite (IHs var replacement Hs).
+    rewrite (IHy (n_lt + var) (shift_lt n_lt 0 replacement) Hy).
+    rewrite (IHn var replacement Hn). reflexivity.
+  - intros E n_beta Ts T_B T_R op_body body IHop IHbody var replacement H.
+    unfold marker_annots_closed in *. simpl in *.
+    apply Forall_app in H as [Hop Hbody].
+    rewrite (IHop var replacement Hop), (IHbody var replacement Hbody). reflexivity.
+  - intros recv Ss arg IHrecv IHarg var replacement H.
+    unfold marker_annots_closed in *. simpl in *.
+    apply Forall_app in H as [Hr Ha].
+    rewrite (IHrecv var replacement Hr), (IHarg var replacement Ha). reflexivity.
+  - intros E m n_beta Ts T_R op_body IHop var replacement H.
+    unfold marker_annots_closed in *. simpl in *.
+    inversion H as [|mt rest Hhead Htail]; subst.
+    destruct Hhead as [_ HLt].
+    rewrite (subst_lt_in_ty_closed0_id T_R var replacement HLt).
+    rewrite (IHop var replacement Htail). reflexivity.
+  - intros m T_B T_R t IH var replacement H.
+    unfold marker_annots_closed in *. simpl in *.
+    inversion H as [|mt rest Hhead Htail]; subst.
+    destruct Hhead as [_ HLt].
+    rewrite (subst_lt_in_ty_closed0_id T_R var replacement HLt).
+    rewrite (IH var replacement Htail). reflexivity.
+  - intros m T_B T_R b IH var replacement H.
+    unfold marker_annots_closed in *. simpl in *.
+    inversion H as [|mt rest Hhead Htail]; subst.
+    destruct Hhead as [_ HLt].
+    rewrite (subst_lt_in_ty_closed0_id T_R var replacement HLt).
+    rewrite (IH var replacement Htail). reflexivity.
+  - intros var replacement H. reflexivity.
+  - intros t ts IHt IHts var replacement H.
+    unfold marker_annots_list_closed in *. simpl in *.
+    apply Forall_app in H as [Ht Hts].
+    rewrite (IHt var replacement Ht), (IHts var replacement Hts). reflexivity.
+Qed.
+
+Lemma marker_annots_subst_list_ty_in_tm_no_local : forall Ss t,
+  marker_annots_no_local t ->
+  marker_annots (subst_list_ty_in_tm Ss t) = marker_annots t.
+Proof.
+  induction Ss as [|S rest IH]; intros t Ht; simpl.
+  - reflexivity.
+  - rewrite (IH _ (marker_annots_no_local_subst_ty_in_tm _ _ _ Ht)).
+    apply marker_annots_subst_ty_in_tm_no_local. exact Ht.
+Qed.
+
+Lemma marker_annots_subst_list_lt_in_tm_no_local : forall lts t,
+  marker_annots_no_local t ->
+  marker_annots (subst_list_lt_in_tm lts t) = marker_annots t.
+Proof.
+  induction lts as [|l rest IH]; intros t Ht; simpl.
+  - reflexivity.
+  - rewrite (IH _ (marker_annots_no_local_subst_lt_in_tm _ _ _ Ht)).
+    apply marker_annots_subst_lt_in_tm_no_local. exact Ht.
+Qed.
+
+Lemma marker_annots_subst_list_ty_in_tm_closed : forall Ss t,
+  marker_annots_closed t ->
+  marker_annots (subst_list_ty_in_tm Ss t) = marker_annots t.
+Proof.
+  induction Ss as [|S rest IH]; intros t Ht; simpl.
+  - reflexivity.
+  - assert (Hsubst : marker_annots_closed (subst_ty_in_tm 0 (shift_ty (List.length rest) 0 S) t)).
+    { unfold marker_annots_closed in *.
+      rewrite marker_annots_subst_ty_in_tm_closed by exact Ht.
+      exact Ht. }
+    rewrite (IH _ Hsubst).
+    apply marker_annots_subst_ty_in_tm_closed. exact Ht.
+Qed.
+
+Lemma marker_annots_subst_list_lt_in_tm_closed : forall lts t,
+  marker_annots_closed t ->
+  marker_annots (subst_list_lt_in_tm lts t) = marker_annots t.
+Proof.
+  induction lts as [|l rest IH]; intros t Ht; simpl.
+  - reflexivity.
+  - assert (Hsubst : marker_annots_closed (subst_lt_in_tm 0 (shift_lt (List.length rest) 0 l) t)).
+    { unfold marker_annots_closed in *.
+      rewrite marker_annots_subst_lt_in_tm_closed by exact Ht.
+      exact Ht. }
+    rewrite (IH _ Hsubst).
+    apply marker_annots_subst_lt_in_tm_closed. exact Ht.
+Qed.
+
+Lemma marker_types_safe_marker_annots_eq : forall t u,
+  marker_annots u = marker_annots t ->
+  marker_types_safe t -> marker_types_safe u.
+Proof.
+  intros t u Hann Hsafe m T U HT HU.
+  unfold marker_types_safe, marker_types_ok in Hsafe.
+  rewrite Hann in HT, HU. eauto.
+Qed.
+
+Lemma marker_types_safe_shift_tm : forall t amount cutoff,
+  marker_types_safe t -> marker_types_safe (shift_tm amount cutoff t).
+Proof.
+  intros t amount cutoff Hsafe.
+  eapply marker_types_safe_marker_annots_eq; [apply marker_annots_shift_tm | exact Hsafe].
+Qed.
+
+Lemma marker_types_safe_subst_list_ty_in_tm_no_local : forall Ss t,
+  marker_annots_no_local t ->
+  marker_types_safe t -> marker_types_safe (subst_list_ty_in_tm Ss t).
+Proof.
+  intros Ss t Hnl Hsafe.
+  eapply marker_types_safe_marker_annots_eq; [apply marker_annots_subst_list_ty_in_tm_no_local |]; eauto.
+Qed.
+
+Lemma marker_types_safe_subst_list_lt_in_tm_no_local : forall lts t,
+  marker_annots_no_local t ->
+  marker_types_safe t -> marker_types_safe (subst_list_lt_in_tm lts t).
+Proof.
+  intros lts t Hnl Hsafe.
+  eapply marker_types_safe_marker_annots_eq; [apply marker_annots_subst_list_lt_in_tm_no_local |]; eauto.
+Qed.
+
+Lemma marker_annots_subst_tm_no_local_incl : forall t var repl,
+  marker_annots_no_local repl ->
+  marker_annots_no_local t ->
+  incl (marker_annots (subst_tm var repl t))
+       (marker_annots repl ++ marker_annots t).
+Proof.
+  apply (term_list_ind
+    (fun t => forall var repl,
+       marker_annots_no_local repl ->
+       marker_annots_no_local t ->
+       incl (marker_annots (subst_tm var repl t))
+            (marker_annots repl ++ marker_annots t))
+    (fun ts => forall var repl,
+       marker_annots_no_local repl ->
+       marker_annots_list_no_local ts ->
+       incl (List.concat (List.map marker_annots (List.map (subst_tm var repl) ts)))
+            (marker_annots repl ++ List.concat (List.map marker_annots ts)))).
+  - intros n var repl Hrepl H p Hp. simpl in *.
+    destruct (Nat.eqb n var); [apply List.in_or_app; left; exact Hp|].
+    destruct (Nat.ltb var n); inversion Hp.
+  - intros t1 t2 IH1 IH2 var repl Hrepl H p Hp.
+    unfold marker_annots_no_local in *. simpl in *.
+    apply Forall_app in H as [H1 H2].
+    apply List.in_app_or in Hp as [Hp | Hp].
+    + specialize (IH1 var repl Hrepl H1 p Hp).
+      repeat rewrite List.in_app_iff in *. tauto.
+    + specialize (IH2 var repl Hrepl H2 p Hp).
+      repeat rewrite List.in_app_iff in *. tauto.
+  - intros body T IH var repl Hrepl H p Hp. simpl in *.
+    specialize (IH (S var) (shift_tm 1 0 repl)
+      (marker_annots_no_local_shift_tm _ _ _ Hrepl) H p Hp).
+    rewrite marker_annots_shift_tm in IH. exact IH.
+  - intros t T IH var repl Hrepl H p Hp. simpl in *.
+    exact (IH var repl Hrepl H p Hp).
+  - intros bound body IH var repl Hrepl H p Hp. simpl in *.
+    specialize (IH var (shift_ty_in_tm 1 0 repl)
+      (marker_annots_no_local_shift_ty_in_tm _ _ _ Hrepl) H p Hp).
+    rewrite (marker_annots_shift_ty_in_tm_no_local repl 1 0 Hrepl) in IH. exact IH.
+  - intros t l IH var repl Hrepl H p Hp. simpl in *.
+    exact (IH var repl Hrepl H p Hp).
+  - intros body IH var repl Hrepl H p Hp. simpl in *.
+    specialize (IH var (shift_lt_in_tm 1 0 repl)
+      (marker_annots_no_local_shift_lt_in_tm _ _ _ Hrepl) H p Hp).
+    rewrite (marker_annots_shift_lt_in_tm_no_local repl 1 0 Hrepl) in IH. exact IH.
+  - intros K l lts Ts ts IH var repl Hrepl H p Hp. simpl in *.
+    rewrite subst_tm_go_eq_map in Hp.
+    unfold marker_annots_no_local in H. fold marker_annots_list_no_local in H.
+    exact (IH var repl Hrepl H p Hp).
+  - intros scrut tag n_lt arity yes no IHs IHy IHn var repl Hrepl H p Hp.
+    unfold marker_annots_no_local in *. simpl in *.
+    repeat rewrite Forall_app in H. destruct H as [Hs [Hy Hn]].
+    repeat rewrite List.in_app_iff in Hp. destruct Hp as [Hp | [Hp | Hp]].
+    + specialize (IHs var repl Hrepl Hs p Hp).
+      repeat rewrite List.in_app_iff in *. tauto.
+    + specialize (IHy (var + arity) (shift_tm arity 0 (shift_lt_in_tm n_lt 0 repl))
+        (marker_annots_no_local_shift_tm _ _ _
+          (marker_annots_no_local_shift_lt_in_tm _ _ _ Hrepl)) Hy p Hp).
+      rewrite marker_annots_shift_tm in IHy.
+      rewrite (marker_annots_shift_lt_in_tm_no_local repl n_lt 0 Hrepl) in IHy.
+      repeat rewrite List.in_app_iff in *. tauto.
+    + specialize (IHn var repl Hrepl Hn p Hp).
+      repeat rewrite List.in_app_iff in *. tauto.
+  - intros E n_beta Ts T_B T_R op_body body IHop IHbody var repl Hrepl H p Hp.
+    unfold marker_annots_no_local in *. simpl in *.
+    apply Forall_app in H as [Hop Hbody].
+    apply List.in_app_or in Hp as [Hp | Hp].
+    + specialize (IHop (var + 2) (shift_tm 2 0 repl)
+        (marker_annots_no_local_shift_tm _ _ _ Hrepl) Hop p Hp).
+      rewrite marker_annots_shift_tm in IHop.
+      repeat rewrite List.in_app_iff in *. tauto.
+    + specialize (IHbody (S var) (shift_tm 1 0 repl)
+        (marker_annots_no_local_shift_tm _ _ _ Hrepl) Hbody p Hp).
+      rewrite marker_annots_shift_tm in IHbody.
+      repeat rewrite List.in_app_iff in *. tauto.
+  - intros recv Ss arg IHrecv IHarg var repl Hrepl H p Hp.
+    unfold marker_annots_no_local in *. simpl in *.
+    apply Forall_app in H as [Hr Ha].
+    apply List.in_app_or in Hp as [Hp | Hp].
+    + specialize (IHrecv var repl Hrepl Hr p Hp).
+      repeat rewrite List.in_app_iff in *. tauto.
+    + specialize (IHarg var repl Hrepl Ha p Hp).
+      repeat rewrite List.in_app_iff in *. tauto.
+  - intros E m n_beta Ts T_R op_body IHop var repl Hrepl H p Hp.
+    unfold marker_annots_no_local in *. simpl in *.
+    inversion H as [|mt rest Hhead Htail]; subst.
+    destruct Hp as [Hp | Hp].
+    + apply List.in_or_app. right. simpl. left. exact Hp.
+    + specialize (IHop (var + 2) (shift_tm 2 0 repl)
+        (marker_annots_no_local_shift_tm _ _ _ Hrepl) Htail p Hp).
+      rewrite marker_annots_shift_tm in IHop.
+      apply List.in_app_or in IHop as [IHop | IHop].
+      * apply List.in_or_app. left. exact IHop.
+      * apply List.in_or_app. right. simpl. right. exact IHop.
+  - intros m T_B T_R t IH var repl Hrepl H p Hp.
+    unfold marker_annots_no_local in *. simpl in *.
+    inversion H as [|mt rest Hhead Htail]; subst.
+    destruct Hp as [Hp | Hp].
+    + apply List.in_or_app. right. simpl. left. exact Hp.
+    + specialize (IH var repl Hrepl Htail p Hp).
+      apply List.in_app_or in IH as [IH | IH].
+      * apply List.in_or_app. left. exact IH.
+      * apply List.in_or_app. right. simpl. right. exact IH.
+  - intros m T_B T_R b IH var repl Hrepl H p Hp.
+    unfold marker_annots_no_local in *. simpl in *.
+    inversion H as [|mt rest Hhead Htail]; subst.
+    destruct Hp as [Hp | Hp].
+    + apply List.in_or_app. right. simpl. left. exact Hp.
+    + specialize (IH (S var) (shift_tm 1 0 repl)
+        (marker_annots_no_local_shift_tm _ _ _ Hrepl) Htail p Hp).
+      rewrite marker_annots_shift_tm in IH.
+      apply List.in_app_or in IH as [IH | IH].
+      * apply List.in_or_app. left. exact IH.
+      * apply List.in_or_app. right. simpl. right. exact IH.
+  - intros var repl Hrepl H p Hp. inversion Hp.
+  - intros t ts IHt IHts var repl Hrepl H p Hp.
+    unfold marker_annots_list_no_local in *. simpl in *.
+    apply Forall_app in H as [Ht Hts].
+    apply List.in_app_or in Hp as [Hp | Hp].
+    + specialize (IHt var repl Hrepl Ht p Hp).
+      repeat rewrite List.in_app_iff in *. tauto.
+    + specialize (IHts var repl Hrepl Hts p Hp).
+      repeat rewrite List.in_app_iff in *. tauto.
+Qed.
+
+Lemma marker_annots_subst_tm_closed_repl_incl : forall t var repl,
+  marker_annots_closed repl ->
+  incl (marker_annots (subst_tm var repl t))
+       (marker_annots repl ++ marker_annots t).
+Proof.
+  apply (term_list_ind
+    (fun t => forall var repl,
+       marker_annots_closed repl ->
+       incl (marker_annots (subst_tm var repl t))
+            (marker_annots repl ++ marker_annots t))
+    (fun ts => forall var repl,
+       marker_annots_closed repl ->
+       incl (List.concat (List.map marker_annots (List.map (subst_tm var repl) ts)))
+            (marker_annots repl ++ List.concat (List.map marker_annots ts)))).
+  - intros n var repl Hrepl p Hp. simpl in *.
+    destruct (Nat.eqb n var); [apply List.in_or_app; left; exact Hp|].
+    destruct (Nat.ltb var n); inversion Hp.
+  - intros t1 t2 IH1 IH2 var repl Hrepl p Hp. simpl in *.
+    apply List.in_app_or in Hp as [Hp | Hp].
+    + specialize (IH1 var repl Hrepl p Hp).
+      repeat rewrite List.in_app_iff in *. tauto.
+    + specialize (IH2 var repl Hrepl p Hp).
+      repeat rewrite List.in_app_iff in *. tauto.
+  - intros body T IH var repl Hrepl p Hp. simpl in *.
+    specialize (IH (S var) (shift_tm 1 0 repl)
+      (marker_annots_closed_shift_tm _ _ _ Hrepl) p Hp).
+    rewrite marker_annots_shift_tm in IH. exact IH.
+  - intros t T IH var repl Hrepl p Hp. simpl in *.
+    exact (IH var repl Hrepl p Hp).
+  - intros bound body IH var repl Hrepl p Hp. simpl in *.
+    specialize (IH var (shift_ty_in_tm 1 0 repl)
+      (marker_annots_closed_shift_ty_in_tm _ _ _ Hrepl) p Hp).
+    rewrite (marker_annots_shift_ty_in_tm_closed repl 1 0 Hrepl) in IH. exact IH.
+  - intros t l IH var repl Hrepl p Hp. simpl in *.
+    exact (IH var repl Hrepl p Hp).
+  - intros body IH var repl Hrepl p Hp. simpl in *.
+    specialize (IH var (shift_lt_in_tm 1 0 repl)
+      (marker_annots_closed_shift_lt_in_tm _ _ _ Hrepl) p Hp).
+    rewrite (marker_annots_shift_lt_in_tm_closed repl 1 0 Hrepl) in IH. exact IH.
+  - intros K l lts Ts ts IH var repl Hrepl p Hp. simpl in *.
+    rewrite subst_tm_go_eq_map in Hp.
+    exact (IH var repl Hrepl p Hp).
+  - intros scrut tag n_lt arity yes no IHs IHy IHn var repl Hrepl p Hp. simpl in *.
+    repeat rewrite List.in_app_iff in Hp. destruct Hp as [Hp | [Hp | Hp]].
+    + specialize (IHs var repl Hrepl p Hp).
+      repeat rewrite List.in_app_iff in *. tauto.
+    + specialize (IHy (var + arity) (shift_tm arity 0 (shift_lt_in_tm n_lt 0 repl))
+        (marker_annots_closed_shift_tm _ _ _
+          (marker_annots_closed_shift_lt_in_tm _ _ _ Hrepl)) p Hp).
+      rewrite marker_annots_shift_tm in IHy.
+      rewrite (marker_annots_shift_lt_in_tm_closed repl n_lt 0 Hrepl) in IHy.
+      repeat rewrite List.in_app_iff in *. tauto.
+    + specialize (IHn var repl Hrepl p Hp).
+      repeat rewrite List.in_app_iff in *. tauto.
+  - intros E n_beta Ts T_B T_R op_body body IHop IHbody var repl Hrepl p Hp. simpl in *.
+    apply List.in_app_or in Hp as [Hp | Hp].
+    + specialize (IHop (var + 2) (shift_tm 2 0 repl)
+        (marker_annots_closed_shift_tm _ _ _ Hrepl) p Hp).
+      rewrite marker_annots_shift_tm in IHop.
+      repeat rewrite List.in_app_iff in *. tauto.
+    + specialize (IHbody (S var) (shift_tm 1 0 repl)
+        (marker_annots_closed_shift_tm _ _ _ Hrepl) p Hp).
+      rewrite marker_annots_shift_tm in IHbody.
+      repeat rewrite List.in_app_iff in *. tauto.
+  - intros recv Ss arg IHrecv IHarg var repl Hrepl p Hp. simpl in *.
+    apply List.in_app_or in Hp as [Hp | Hp].
+    + specialize (IHrecv var repl Hrepl p Hp).
+      repeat rewrite List.in_app_iff in *. tauto.
+    + specialize (IHarg var repl Hrepl p Hp).
+      repeat rewrite List.in_app_iff in *. tauto.
+  - intros E m n_beta Ts T_R op_body IHop var repl Hrepl p Hp. simpl in *.
+    destruct Hp as [Hp | Hp].
+    + apply List.in_or_app. right. simpl. left. exact Hp.
+    + specialize (IHop (var + 2) (shift_tm 2 0 repl)
+        (marker_annots_closed_shift_tm _ _ _ Hrepl) p Hp).
+      rewrite marker_annots_shift_tm in IHop.
+      apply List.in_app_or in IHop as [IHop | IHop].
+      * apply List.in_or_app. left. exact IHop.
+      * apply List.in_or_app. right. simpl. right. exact IHop.
+  - intros m T_B T_R t IH var repl Hrepl p Hp. simpl in *.
+    destruct Hp as [Hp | Hp].
+    + apply List.in_or_app. right. simpl. left. exact Hp.
+    + specialize (IH var repl Hrepl p Hp).
+      apply List.in_app_or in IH as [IH | IH].
+      * apply List.in_or_app. left. exact IH.
+      * apply List.in_or_app. right. simpl. right. exact IH.
+  - intros m T_B T_R b IH var repl Hrepl p Hp. simpl in *.
+    destruct Hp as [Hp | Hp].
+    + apply List.in_or_app. right. simpl. left. exact Hp.
+    + specialize (IH (S var) (shift_tm 1 0 repl)
+        (marker_annots_closed_shift_tm _ _ _ Hrepl) p Hp).
+      rewrite marker_annots_shift_tm in IH.
+      apply List.in_app_or in IH as [IH | IH].
+      * apply List.in_or_app. left. exact IH.
+      * apply List.in_or_app. right. simpl. right. exact IH.
+  - intros var repl Hrepl p Hp. inversion Hp.
+  - intros t ts IHt IHts var repl Hrepl p Hp. simpl in *.
+    apply List.in_app_or in Hp as [Hp | Hp].
+    + specialize (IHt var repl Hrepl p Hp).
+      repeat rewrite List.in_app_iff in *. tauto.
+    + specialize (IHts var repl Hrepl p Hp).
+      repeat rewrite List.in_app_iff in *. tauto.
+Qed.
+
+Lemma marker_annots_subst_list_tm_no_local_incl : forall vs t,
+  Forall marker_annots_no_local vs ->
+  marker_annots_no_local t ->
+  incl (marker_annots (subst_list_tm vs t))
+       (List.concat (List.map marker_annots vs) ++ marker_annots t).
+Proof.
+  induction vs as [|v rest IH]; intros t Hvs Ht p Hp; simpl in *.
+  - exact Hp.
+  - inversion Hvs as [|v0 rest0 Hv Hrest Heq]; subst.
+    specialize (IH (subst_tm 0 (shift_tm (List.length rest) 0 v) t) Hrest
+      (marker_annots_no_local_subst_tm _ _ _
+        (marker_annots_no_local_shift_tm _ _ _ Hv) Ht) p Hp).
+    apply List.in_app_or in IH as [HinRest | HinSubst].
+    + repeat rewrite List.in_app_iff in *. tauto.
+    + pose proof (marker_annots_subst_tm_no_local_incl t 0
+        (shift_tm (List.length rest) 0 v)
+        (marker_annots_no_local_shift_tm _ _ _ Hv) Ht p HinSubst) as Hsingle.
+      rewrite marker_annots_shift_tm in Hsingle.
+      repeat rewrite List.in_app_iff in *. tauto.
+Qed.
+
+Lemma marker_annots_subst_list_tm_closed_repl_incl : forall vs t,
+  Forall marker_annots_closed vs ->
+  incl (marker_annots (subst_list_tm vs t))
+       (List.concat (List.map marker_annots vs) ++ marker_annots t).
+Proof.
+  induction vs as [|v rest IH]; intros t Hvs p Hp; simpl in *.
+  - exact Hp.
+  - inversion Hvs as [|v0 rest0 Hv Hrest Heq]; subst.
+    specialize (IH (subst_tm 0 (shift_tm (List.length rest) 0 v) t) Hrest p Hp).
+    apply List.in_app_or in IH as [HinRest | HinSubst].
+    + repeat rewrite List.in_app_iff in *. tauto.
+    + pose proof (marker_annots_subst_tm_closed_repl_incl t 0
+        (shift_tm (List.length rest) 0 v)
+        (marker_annots_closed_shift_tm _ _ _ Hv) p HinSubst) as Hsingle.
+      rewrite marker_annots_shift_tm in Hsingle.
+      repeat rewrite List.in_app_iff in *. tauto.
+Qed.
+
+Lemma marker_annots_no_local_incl : forall sub whole,
+  incl (marker_annots sub) (marker_annots whole) ->
+  marker_annots_no_local whole -> marker_annots_no_local sub.
+Proof.
+  intros sub whole Hincl Hwhole.
+  unfold marker_annots_no_local in *.
+  apply Forall_forall. intros mt Hmt.
+  apply Forall_forall with (x := mt) in Hwhole; [exact Hwhole | apply Hincl; exact Hmt].
+Qed.
+
+Lemma marker_annots_closed_incl : forall sub whole,
+  incl (marker_annots sub) (marker_annots whole) ->
+  marker_annots_closed whole -> marker_annots_closed sub.
+Proof.
+  intros sub whole Hincl Hwhole.
+  unfold marker_annots_closed in *.
+  apply Forall_forall. intros mt Hmt.
+  apply Forall_forall with (x := mt) in Hwhole; [exact Hwhole | apply Hincl; exact Hmt].
+Qed.
+
+Lemma marker_annots_closed_cons_incl : forall t m T source,
+  ty_ty_closed 0 T ->
+  ty_lt_closed 0 T ->
+  marker_annots_closed source ->
+  incl (marker_annots t) ((m, T) :: marker_annots source) ->
+  marker_annots_closed t.
+Proof.
+  intros t m T source HTy HLt Hsource Hincl.
+  unfold marker_annots_closed in *.
+  apply Forall_forall. intros mt Hmt.
+  specialize (Hincl mt Hmt) as Hin.
+  destruct mt as [m0 T0].
+  simpl in Hin |- *. destruct Hin as [Hin | Hin].
+  - inversion Hin; subst. simpl. split; assumption.
+  - exact (proj1 (Forall_forall _ _) Hsource (m0, T0) Hin).
+Qed.
+
+Lemma marker_annots_closed_concat : forall ts,
+  Forall marker_annots_closed ts ->
+  Forall (fun mt => ty_ty_closed 0 (snd mt) /\ ty_lt_closed 0 (snd mt))
+    (List.concat (List.map marker_annots ts)).
+Proof.
+  induction ts as [|t ts IH]; intros Hts; simpl.
+  - constructor.
+  - inversion Hts as [|t0 ts0 Ht Hrest Heq]; subst.
+    apply Forall_app. split.
+    + exact Ht.
+    + apply IH. exact Hrest.
+Qed.
+
+Lemma marker_annots_closed_subst_tm : forall t var repl,
+  marker_annots_closed repl ->
+  marker_annots_closed t ->
+  marker_annots_closed (subst_tm var repl t).
+Proof.
+  intros t var repl Hrepl Ht.
+  unfold marker_annots_closed in *.
+  apply Forall_forall. intros mt Hmt.
+  pose proof (marker_annots_subst_tm_closed_repl_incl t var repl Hrepl mt Hmt) as Hin.
+  apply List.in_app_or in Hin as [Hin | Hin].
+  - exact (proj1 (Forall_forall _ _) Hrepl mt Hin).
+  - exact (proj1 (Forall_forall _ _) Ht mt Hin).
+Qed.
+
+Lemma marker_annots_closed_subst_list_tm : forall vs t,
+  Forall marker_annots_closed vs ->
+  marker_annots_closed t ->
+  marker_annots_closed (subst_list_tm vs t).
+Proof.
+  intros vs t Hvs Ht.
+  unfold marker_annots_closed in *.
+  apply Forall_forall. intros mt Hmt.
+  pose proof (marker_annots_subst_list_tm_closed_repl_incl vs t Hvs mt Hmt) as Hin.
+  apply List.in_app_or in Hin as [Hin | Hin].
+  - exact (proj1 (Forall_forall _ _) (marker_annots_closed_concat _ Hvs) mt Hin).
+  - exact (proj1 (Forall_forall _ _) Ht mt Hin).
+Qed.
+
+Lemma marker_annots_closed_subst_list_ty_in_tm : forall Ss t,
+  marker_annots_closed t ->
+  marker_annots_closed (subst_list_ty_in_tm Ss t).
+Proof.
+  intros Ss t Ht. unfold marker_annots_closed in *.
+  rewrite marker_annots_subst_list_ty_in_tm_closed by exact Ht. exact Ht.
+Qed.
+
+Lemma marker_annots_closed_subst_list_lt_in_tm : forall lts t,
+  marker_annots_closed t ->
+  marker_annots_closed (subst_list_lt_in_tm lts t).
+Proof.
+  intros lts t Ht. unfold marker_annots_closed in *.
+  rewrite marker_annots_subst_list_lt_in_tm_closed by exact Ht. exact Ht.
+Qed.
+
+Lemma marker_annots_list_no_local_Forall : forall ts,
+  marker_annots_list_no_local ts -> Forall marker_annots_no_local ts.
+Proof.
+  induction ts as [|t ts IH]; intros H; constructor.
+  - unfold marker_annots_list_no_local, marker_annots_no_local in *.
+    simpl in H. apply Forall_app in H as [Ht _]. exact Ht.
+  - apply IH. unfold marker_annots_list_no_local in *.
+    simpl in H. apply Forall_app in H as [_ Hts]. exact Hts.
+Qed.
+
+Lemma marker_annots_list_closed_Forall : forall ts,
+  marker_annots_list_closed ts -> Forall marker_annots_closed ts.
+Proof.
+  induction ts as [|t ts IH]; intros H; constructor.
+  - unfold marker_annots_list_closed, marker_annots_closed in *.
+    simpl in H. apply Forall_app in H as [Ht _]. exact Ht.
+  - apply IH. unfold marker_annots_list_closed in *.
+    simpl in H. apply Forall_app in H as [_ Hts]. exact Hts.
+Qed.
+
+Lemma marker_annots_beta_incl_no_local : forall body T v,
+  marker_annots_no_local body ->
+  marker_annots_no_local v ->
+  incl (marker_annots (subst_tm 0 v body))
+       (marker_annots (term_app (term_lam body T) v)).
+Proof.
+  intros body T v Hbody Hv p Hp.
+  pose proof (marker_annots_subst_tm_no_local_incl body 0 v Hv Hbody p Hp) as Hincl.
+  simpl. repeat rewrite List.in_app_iff in *. tauto.
+Qed.
+
+Lemma marker_annots_tybeta_incl_no_local : forall bound body T,
+  marker_annots_no_local body ->
+  incl (marker_annots (subst_ty_in_tm 0 T body))
+       (marker_annots (term_ty_app (term_ty_lam bound body) T)).
+Proof.
+  intros bound body T Hbody p Hp. simpl.
+  rewrite marker_annots_subst_ty_in_tm_no_local in Hp; [exact Hp | exact Hbody].
+Qed.
+
+Lemma marker_annots_ltbeta_incl_no_local : forall body l,
+  marker_annots_no_local body ->
+  incl (marker_annots (subst_lt_in_tm 0 l body))
+       (marker_annots (term_lt_app (term_lt_lam body) l)).
+Proof.
+  intros body l Hbody p Hp. simpl.
+  rewrite marker_annots_subst_lt_in_tm_no_local in Hp; [exact Hp | exact Hbody].
+Qed.
+
+Lemma marker_annots_match_yes_incl_no_local : forall K l lts Ts vs n_lt yes_body no_body,
+  marker_annots_list_no_local vs ->
+  marker_annots_no_local yes_body ->
+  incl (marker_annots (subst_list_tm vs (subst_list_lt_in_tm lts yes_body)))
+       (marker_annots (term_match (term_ctor K l lts Ts vs) K n_lt (List.length vs) yes_body no_body)).
+Proof.
+  intros K l lts Ts vs n_lt yes_body no_body Hvs Hyes p Hp.
+  pose proof (marker_annots_subst_list_tm_no_local_incl vs
+    (subst_list_lt_in_tm lts yes_body)
+    (marker_annots_list_no_local_Forall _ Hvs)
+    (marker_annots_no_local_subst_list_lt_in_tm _ _ Hyes) p Hp) as Hincl.
+  rewrite marker_annots_subst_list_lt_in_tm_no_local in Hincl; [|exact Hyes].
+  simpl. repeat rewrite List.in_app_iff in *. tauto.
+Qed.
+
+Lemma marker_annots_match_no_incl : forall K K' l lts Ts vs n_lt arity yes_body no_body,
+  incl (marker_annots no_body)
+       (marker_annots (term_match (term_ctor K' l lts Ts vs) K n_lt arity yes_body no_body)).
+Proof.
+  intros K K' l lts Ts vs n_lt arity yes_body no_body p Hp.
+  simpl. repeat rewrite List.in_app_iff. tauto.
+Qed.
+
+Lemma marker_annots_return_incl : forall m T_B T_R v,
+  incl (marker_annots v) (marker_annots (term_handler_m m T_B T_R v)).
+Proof.
+  intros m T_B T_R v p Hp. simpl. right. exact Hp.
+Qed.
+
+Lemma marker_annots_resume_incl_no_local : forall m T_B T_R b v,
+  marker_annots_no_local b ->
+  marker_annots_no_local v ->
+  incl (marker_annots (term_handler_m m T_B T_R (subst_tm 0 v b)))
+       (marker_annots (term_app (term_resume m T_B T_R b) v)).
+Proof.
+  intros m T_B T_R b v Hb Hv p Hp. simpl in Hp |- *.
+  destruct Hp as [Hp | Hp].
+  - left. exact Hp.
+  - pose proof (marker_annots_subst_tm_no_local_incl b 0 v Hv Hb p Hp) as Hincl.
+    repeat rewrite List.in_app_iff in *. simpl in *. tauto.
+Qed.
+
+Lemma marker_annots_beta_incl_closed : forall body T v,
+  marker_annots_closed v ->
+  incl (marker_annots (subst_tm 0 v body))
+       (marker_annots (term_app (term_lam body T) v)).
+Proof.
+  intros body T v Hv p Hp.
+  pose proof (marker_annots_subst_tm_closed_repl_incl body 0 v Hv p Hp) as Hincl.
+  simpl. repeat rewrite List.in_app_iff in *. tauto.
+Qed.
+
+Lemma marker_annots_tybeta_incl_closed : forall bound body T,
+  marker_annots_closed body ->
+  incl (marker_annots (subst_ty_in_tm 0 T body))
+       (marker_annots (term_ty_app (term_ty_lam bound body) T)).
+Proof.
+  intros bound body T Hbody p Hp. simpl.
+  rewrite marker_annots_subst_ty_in_tm_closed in Hp; [exact Hp | exact Hbody].
+Qed.
+
+Lemma marker_annots_ltbeta_incl_closed : forall body l,
+  marker_annots_closed body ->
+  incl (marker_annots (subst_lt_in_tm 0 l body))
+       (marker_annots (term_lt_app (term_lt_lam body) l)).
+Proof.
+  intros body l Hbody p Hp. simpl.
+  rewrite marker_annots_subst_lt_in_tm_closed in Hp; [exact Hp | exact Hbody].
+Qed.
+
+Lemma marker_annots_match_yes_incl_closed : forall K l lts Ts vs n_lt yes_body no_body,
+  marker_annots_list_closed vs ->
+  marker_annots_closed yes_body ->
+  incl (marker_annots (subst_list_tm vs (subst_list_lt_in_tm lts yes_body)))
+       (marker_annots (term_match (term_ctor K l lts Ts vs) K n_lt (List.length vs) yes_body no_body)).
+Proof.
+  intros K l lts Ts vs n_lt yes_body no_body Hvs Hyes p Hp.
+  pose proof (marker_annots_subst_list_tm_closed_repl_incl vs
+    (subst_list_lt_in_tm lts yes_body)
+    (marker_annots_list_closed_Forall _ Hvs) p Hp) as Hincl.
+  rewrite marker_annots_subst_list_lt_in_tm_closed in Hincl; [|exact Hyes].
+  simpl. repeat rewrite List.in_app_iff in *. tauto.
+Qed.
+
+Lemma marker_annots_resume_incl_closed : forall m T_B T_R b v,
+  marker_annots_closed v ->
+  incl (marker_annots (term_handler_m m T_B T_R (subst_tm 0 v b)))
+       (marker_annots (term_app (term_resume m T_B T_R b) v)).
+Proof.
+  intros m T_B T_R b v Hv p Hp. simpl in Hp |- *.
+  destruct Hp as [Hp | Hp].
+  - left. exact Hp.
+  - pose proof (marker_annots_subst_tm_closed_repl_incl b 0 v Hv p Hp) as Hincl.
+    repeat rewrite List.in_app_iff in *. simpl in *. tauto.
+Qed.
+
+Lemma head_step_marker_annots_incl_no_local_with_perform :
+  forall r r',
+    r -->h r' ->
+    marker_annots_no_local r ->
+    (forall E_tag m n_beta Ts T_B T_R op_body Ss v P,
+      value v -> pure_ectx_m m P ->
+      marker_annots_no_local
+        (term_handler_m m T_B T_R
+          (plug P (term_perform (term_cap E_tag m n_beta Ts T_R op_body) Ss v))) ->
+      incl
+        (marker_annots
+          (subst_list_tm [v; term_resume m T_B T_R (plug (shift_ectx_tm 1 0 P) (term_var 0))]
+            (subst_list_ty_in_tm Ss op_body)))
+        (marker_annots
+          (term_handler_m m T_B T_R
+            (plug P (term_perform (term_cap E_tag m n_beta Ts T_R op_body) Ss v))))) ->
+    incl (marker_annots r') (marker_annots r).
+Proof.
+  intros r r' Hstep Hnl Hperform.
+  inversion Hstep; subst.
+  - (* H_Beta *)
+    simpl in Hnl. apply Forall_app in Hnl as [Hbody Hv].
+    apply marker_annots_beta_incl_no_local; assumption.
+  - (* H_TyBeta *)
+    apply marker_annots_tybeta_incl_no_local. exact Hnl.
+  - (* H_LtBeta *)
+    apply marker_annots_ltbeta_incl_no_local. exact Hnl.
+  - (* H_MatchYes *)
+    simpl in Hnl. apply Forall_app in Hnl as [Hvs Hyn].
+    apply Forall_app in Hyn as [Hyes _].
+    apply marker_annots_match_yes_incl_no_local; assumption.
+  - (* H_MatchNo *)
+    apply marker_annots_match_no_incl.
+  - (* H_Return *)
+    apply marker_annots_return_incl.
+  - (* H_Perform *)
+    eapply Hperform; eauto.
+  - (* H_Resume *)
+    simpl in Hnl. apply Forall_app in Hnl as [Hresume Hv].
+    inversion Hresume as [|mt rest Hhead Hb]; subst.
+    apply marker_annots_resume_incl_no_local; assumption.
+Qed.
+
+Lemma head_step_preserves_marker_types_safe_no_local_with_perform :
+  forall r r',
+    r -->h r' ->
+    marker_annots_no_local r ->
+    marker_types_safe r ->
+    (forall E_tag m n_beta Ts T_B T_R op_body Ss v P,
+      value v -> pure_ectx_m m P ->
+      marker_annots_no_local
+        (term_handler_m m T_B T_R
+          (plug P (term_perform (term_cap E_tag m n_beta Ts T_R op_body) Ss v))) ->
+      marker_types_safe
+        (term_handler_m m T_B T_R
+          (plug P (term_perform (term_cap E_tag m n_beta Ts T_R op_body) Ss v))) ->
+      marker_types_safe
+        (subst_list_tm [v; term_resume m T_B T_R (plug (shift_ectx_tm 1 0 P) (term_var 0))]
+          (subst_list_ty_in_tm Ss op_body))) ->
+    marker_types_safe r'.
+Proof.
+  intros r r' Hstep Hnl Hsafe Hperform.
+  inversion Hstep; subst.
+  - (* H_Beta *)
+    simpl in Hnl. apply Forall_app in Hnl as [Hbody Hv].
+    eapply marker_types_safe_incl; [apply marker_annots_beta_incl_no_local; eauto | exact Hsafe].
+  - (* H_TyBeta *)
+    eapply marker_types_safe_incl; [apply marker_annots_tybeta_incl_no_local; exact Hnl | exact Hsafe].
+  - (* H_LtBeta *)
+    eapply marker_types_safe_incl; [apply marker_annots_ltbeta_incl_no_local; exact Hnl | exact Hsafe].
+  - (* H_MatchYes *)
+    simpl in Hnl. apply Forall_app in Hnl as [Hvs Hyn].
+    apply Forall_app in Hyn as [Hyes _].
+    eapply marker_types_safe_incl; [apply marker_annots_match_yes_incl_no_local; eauto | exact Hsafe].
+  - (* H_MatchNo *)
+    eapply marker_types_safe_incl; [apply marker_annots_match_no_incl | exact Hsafe].
+  - (* H_Return *)
+    eapply marker_types_safe_incl; [apply marker_annots_return_incl | exact Hsafe].
+  - (* H_Perform *)
+    eapply Hperform; eauto.
+  - (* H_Resume *)
+    simpl in Hnl. apply Forall_app in Hnl as [Hresume Hv].
+    inversion Hresume as [|mt rest Hhead Hb]; subst.
+    eapply marker_types_safe_incl; [apply marker_annots_resume_incl_no_local; eauto | exact Hsafe].
+Qed.
+
+Lemma incl_app_compat_local : forall (A : Type) (xs xs' ys ys' : list A),
+  incl xs xs' -> incl ys ys' -> incl (xs ++ ys) (xs' ++ ys').
+Proof.
+  intros A xs xs' ys ys' Hxs Hys p Hp.
+  apply List.in_app_or in Hp as [Hp | Hp].
+  - apply List.in_or_app. left. apply Hxs. exact Hp.
+  - apply List.in_or_app. right. apply Hys. exact Hp.
+Qed.
+
+Lemma incl_cons_same_local : forall (A : Type) (x : A) xs ys,
+  incl xs ys -> incl (x :: xs) (x :: ys).
+Proof.
+  intros A x xs ys H p Hp. simpl in Hp |- *.
+  destruct Hp as [Hp | Hp]; [left; exact Hp | right; apply H; exact Hp].
+Qed.
+
+Lemma marker_annots_ctor_replace_incl : forall vs t t' ts,
+  incl (marker_annots t') (marker_annots t) ->
+  incl (List.concat (List.map marker_annots (vs ++ t' :: ts)))
+       (List.concat (List.map marker_annots (vs ++ t :: ts))).
+Proof.
+  induction vs as [|v vs IH]; intros t t' ts Hincl.
+  - simpl. apply incl_app_compat_local; [exact Hincl | apply incl_refl].
+  - simpl. apply incl_app_compat_local; [apply incl_refl | apply IH; exact Hincl].
+Qed.
+
+Lemma marker_annots_ctor_replace_incl_cons : forall vs t t' ts new,
+  incl (marker_annots t') (new :: marker_annots t) ->
+  incl (List.concat (List.map marker_annots (vs ++ t' :: ts)))
+       (new :: List.concat (List.map marker_annots (vs ++ t :: ts))).
+Proof.
+  induction vs as [|v vs IH]; intros t t' ts new Hincl p Hp; simpl in *.
+  - apply List.in_app_or in Hp as [Hp | Hp].
+    + specialize (Hincl p Hp). simpl in Hincl. destruct Hincl as [Hnew | Hold].
+      * left. exact Hnew.
+      * right. apply List.in_or_app. left. exact Hold.
+    + right. apply List.in_or_app. right. exact Hp.
+  - apply List.in_app_or in Hp as [Hp | Hp].
+    + right. apply List.in_or_app. left. exact Hp.
+    + specialize (IH t t' ts new Hincl p Hp). simpl in IH. destruct IH as [Hnew | Hold].
+      * left. exact Hnew.
+      * right. apply List.in_or_app. right. exact Hold.
+Qed.
+
+Lemma marker_annots_plug_replace_incl : forall E r r',
+  incl (marker_annots r') (marker_annots r) ->
+  incl (marker_annots (plug E r')) (marker_annots (plug E r)).
+Proof.
+  induction E; intros r r' Hincl; simpl.
+  - exact Hincl.
+  - apply incl_app_compat_local; [apply IHE; exact Hincl | apply incl_refl].
+  - apply incl_app_compat_local; [apply incl_refl | apply IHE; exact Hincl].
+  - apply IHE. exact Hincl.
+  - apply IHE. exact Hincl.
+  - apply marker_annots_ctor_replace_incl. apply IHE. exact Hincl.
+  - apply incl_app_compat_local; [apply IHE; exact Hincl | apply incl_refl].
+  - apply incl_cons_same_local. apply IHE. exact Hincl.
+  - apply incl_app_compat_local; [apply IHE; exact Hincl | apply incl_refl].
+  - apply incl_app_compat_local; [apply incl_refl | apply IHE; exact Hincl].
+Qed.
+
+Lemma marker_annots_plug_replace_incl_cons : forall E r r' new,
+  incl (marker_annots r') (new :: marker_annots r) ->
+  incl (marker_annots (plug E r')) (new :: marker_annots (plug E r)).
+Proof.
+  induction E; intros r r' new Hincl p Hp; simpl in *.
+  - apply Hincl. exact Hp.
+  - apply List.in_app_or in Hp as [Hp | Hp].
+    + specialize (IHE r r' new Hincl p Hp). simpl in IHE. destruct IHE as [Hnew | Hold].
+      * left. exact Hnew.
+      * right. apply List.in_or_app. left. exact Hold.
+    + right. apply List.in_or_app. right. exact Hp.
+  - apply List.in_app_or in Hp as [Hp | Hp].
+    + right. apply List.in_or_app. left. exact Hp.
+    + specialize (IHE r r' new Hincl p Hp). simpl in IHE. destruct IHE as [Hnew | Hold].
+      * left. exact Hnew.
+      * right. apply List.in_or_app. right. exact Hold.
+  - exact (IHE r r' new Hincl p Hp).
+  - exact (IHE r r' new Hincl p Hp).
+  - exact (marker_annots_ctor_replace_incl_cons _ _ _ _ _
+      (IHE r r' new Hincl) p Hp).
+  - apply List.in_app_or in Hp as [Hp | Hp].
+    + specialize (IHE r r' new Hincl p Hp). simpl in IHE. destruct IHE as [Hnew | Hold].
+      * left. exact Hnew.
+      * right. apply List.in_or_app. left. exact Hold.
+    + right. apply List.in_or_app. right. exact Hp.
+  - destruct Hp as [Hp | Hp].
+    + right. left. exact Hp.
+    + specialize (IHE r r' new Hincl p Hp). simpl in IHE. destruct IHE as [Hnew | Hold].
+      * left. exact Hnew.
+      * right. right. exact Hold.
+  - apply List.in_app_or in Hp as [Hp | Hp].
+    + specialize (IHE r r' new Hincl p Hp). simpl in IHE. destruct IHE as [Hnew | Hold].
+      * left. exact Hnew.
+      * right. apply List.in_or_app. left. exact Hold.
+    + right. apply List.in_or_app. right. exact Hp.
+  - apply List.in_app_or in Hp as [Hp | Hp].
+    + right. apply List.in_or_app. left. exact Hp.
+    + specialize (IHE r r' new Hincl p Hp). simpl in IHE. destruct IHE as [Hnew | Hold].
+      * left. exact Hnew.
+      * right. apply List.in_or_app. right. exact Hold.
+Qed.
+
+Lemma marker_annots_plug_var_incl : forall E r n,
+  incl (marker_annots (plug E (term_var n))) (marker_annots (plug E r)).
+Proof.
+  intros E r n. apply marker_annots_plug_replace_incl.
+  intros p Hp. inversion Hp.
+Qed.
+
+Lemma marker_annots_shift_ectx_tm_plug_var_incl : forall E r amount cutoff n,
+  incl (marker_annots (plug (shift_ectx_tm amount cutoff E) (term_var n)))
+       (marker_annots (plug E r)).
+Proof.
+  intros E r amount cutoff n p Hp.
+  rewrite marker_annots_shift_ectx_tm in Hp.
+  eapply marker_annots_plug_var_incl. exact Hp.
+Qed.
+
+Lemma marker_types_safe_plug_replace_incl : forall E r r',
+  incl (marker_annots r') (marker_annots r) ->
+  marker_types_safe (plug E r) ->
+  marker_types_safe (plug E r').
+Proof.
+  intros E r r' Hincl Hsafe.
+  eapply marker_types_safe_incl; [apply marker_annots_plug_replace_incl; exact Hincl | exact Hsafe].
+Qed.
+
+Lemma markers_in_ctor_eq : forall K l lts Ts ts,
+  markers_in (term_ctor K l lts Ts ts) = markers_in_list ts.
+Proof.
+  intros K l lts Ts ts. simpl.
+  induction ts as [|u rest IH]; simpl; [reflexivity | rewrite IH; reflexivity].
+Qed.
+
+Lemma marker_annots_marker_in : forall t m T,
+  In (m, T) (marker_annots t) -> In m (markers_in t).
+Proof.
+  apply (term_list_ind
+    (fun t => forall m T, In (m, T) (marker_annots t) -> In m (markers_in t))
+    (fun ts => forall m T,
+       In (m, T) (List.concat (List.map marker_annots ts)) ->
+       In m (markers_in_list ts))).
+  - intros n m T H. inversion H.
+  - intros t1 t2 IH1 IH2 m T H. simpl in *.
+    apply List.in_app_or in H as [H | H].
+    + apply List.in_or_app. left. apply IH1 with (T := T). exact H.
+    + apply List.in_or_app. right. apply IH2 with (T := T). exact H.
+  - intros body T0 IH m T H. simpl in *. apply IH with (T := T). exact H.
+  - intros t T0 IH m T H. simpl in *. apply IH with (T := T). exact H.
+  - intros bound body IH m T H. simpl in *. apply IH with (T := T). exact H.
+  - intros t l IH m T H. simpl in *. apply IH with (T := T). exact H.
+  - intros body IH m T H. simpl in *. apply IH with (T := T). exact H.
+  - intros K l lts Ts ts IH m T H. rewrite markers_in_ctor_eq. apply IH with (T := T). exact H.
+  - intros scrut tag n_lt arity yes no IHs IHy IHn m T H. simpl in *.
+    repeat rewrite List.in_app_iff in H. destruct H as [H | [H | H]].
+    + apply List.in_or_app. left. apply IHs with (T := T). exact H.
+    + apply List.in_or_app. right. apply List.in_or_app. left. apply IHy with (T := T). exact H.
+    + apply List.in_or_app. right. apply List.in_or_app. right. apply IHn with (T := T). exact H.
+  - intros E n_beta Ts T_B T_R op_body body IHop IHbody m T H. simpl in *.
+    apply List.in_app_or in H as [H | H].
+    + apply List.in_or_app. left. apply IHop with (T := T). exact H.
+    + apply List.in_or_app. right. apply IHbody with (T := T). exact H.
+  - intros recv Ss arg IHrecv IHarg m T H. simpl in *.
+    apply List.in_app_or in H as [H | H].
+    + apply List.in_or_app. left. apply IHrecv with (T := T). exact H.
+    + apply List.in_or_app. right. apply IHarg with (T := T). exact H.
+  - intros E m0 n_beta Ts T_R op_body IHop m T H. simpl in *.
+    destruct H as [H | H].
+    + injection H; intros; subst. left. reflexivity.
+    + right. apply IHop with (T := T). exact H.
+  - intros m0 T_B T_R body IH m T H. simpl in *.
+    destruct H as [H | H].
+    + injection H; intros; subst. left. reflexivity.
+    + right. apply IH with (T := T). exact H.
+  - intros m0 T_B T_R body IH m T H. simpl in *.
+    destruct H as [H | H].
+    + injection H; intros; subst. left. reflexivity.
+    + right. apply IH with (T := T). exact H.
+  - intros m T H. inversion H.
+  - intros t ts IHt IHts m T H. simpl in *.
+    apply List.in_app_or in H as [H | H].
+    + apply List.in_or_app. left. apply IHt with (T := T). exact H.
+    + apply List.in_or_app. right. apply IHts with (T := T). exact H.
+Qed.
+
+Lemma marker_types_safe_fresh_cons_incl : forall source t m T,
+  ~ In m (markers_in source) ->
+  marker_types_safe source ->
+  incl (marker_annots t) ((m, T) :: marker_annots source) ->
+  marker_types_safe t.
+Proof.
+  intros source t m T Hfresh Hsafe Hincl m0 U V HU HV.
+  specialize (Hincl _ HU) as HU'.
+  specialize (Hincl _ HV) as HV'.
+  simpl in HU', HV'.
+  destruct HU' as [HU' | HU']; destruct HV' as [HV' | HV'].
+  - injection HU'; injection HV'; intros; subst. reflexivity.
+  - injection HU'; intros; subst. exfalso. apply Hfresh.
+    eapply marker_annots_marker_in. exact HV'.
+  - injection HV'; intros; subst. exfalso. apply Hfresh.
+    eapply marker_annots_marker_in. exact HU'.
+  - eapply Hsafe; eauto.
+Qed.
+
+Lemma marker_annots_closed_cap : forall E m n_beta Ts T_R op_body,
+  ty_ty_closed 0 T_R ->
+  ty_lt_closed 0 T_R ->
+  marker_annots_closed op_body ->
+  marker_annots_closed (term_cap E m n_beta Ts T_R op_body).
+Proof.
+  intros E m n_beta Ts T_R op_body HTy HLt Hop.
+  unfold marker_annots_closed in *. simpl. constructor.
+  - simpl. split; assumption.
+  - exact Hop.
+Qed.
+
+Lemma marker_annots_handle_alloc_redex_incl_closed :
+  forall E_tag n_beta Ts T_B T_R op_body body m,
+    ty_ty_closed 0 T_R ->
+    ty_lt_closed 0 T_R ->
+    marker_annots_closed op_body ->
+    incl
+      (marker_annots
+        (term_handler_m m T_B T_R
+          (subst_tm 0 (term_cap E_tag m n_beta Ts T_R op_body) body)))
+      ((m, T_R) :: marker_annots (term_handle E_tag n_beta Ts T_B T_R op_body body)).
+Proof.
+  intros E_tag n_beta Ts T_B T_R op_body body m HTy HLt Hop p Hp.
+  simpl in Hp |- *.
+  destruct Hp as [Hp | Hp].
+  - left. exact Hp.
+  - pose proof (marker_annots_closed_cap E_tag m n_beta Ts T_R op_body HTy HLt Hop) as Hcap.
+    pose proof (marker_annots_subst_tm_closed_repl_incl body 0
+      (term_cap E_tag m n_beta Ts T_R op_body) Hcap p Hp) as Hincl.
+    simpl in Hincl. repeat rewrite List.in_app_iff in *. tauto.
+Qed.
+
+Lemma marker_types_safe_handle_alloc_closed :
+  forall E E_tag n_beta Ts T_B T_R op_body body m,
+    ~ In m (markers_in (plug E (term_handle E_tag n_beta Ts T_B T_R op_body body))) ->
+    ty_ty_closed 0 T_R ->
+    ty_lt_closed 0 T_R ->
+    marker_annots_closed op_body ->
+    marker_types_safe (plug E (term_handle E_tag n_beta Ts T_B T_R op_body body)) ->
+    marker_types_safe
+      (plug E
+        (term_handler_m m T_B T_R
+          (subst_tm 0 (term_cap E_tag m n_beta Ts T_R op_body) body))).
+Proof.
+  intros E E_tag n_beta Ts T_B T_R op_body body m Hfresh HTy HLt Hop Hsafe.
+  eapply marker_types_safe_fresh_cons_incl with
+    (source := plug E (term_handle E_tag n_beta Ts T_B T_R op_body body))
+    (m := m) (T := T_R); eauto.
+  apply marker_annots_plug_replace_incl_cons.
+  apply marker_annots_handle_alloc_redex_incl_closed; assumption.
+Qed.
+
+Lemma marker_types_safe_cap_fresh : forall E m n_beta Ts T_R op_body,
+  ~ In m (markers_in op_body) ->
+  marker_types_safe op_body ->
+  marker_types_safe (term_cap E m n_beta Ts T_R op_body).
+Proof.
+  intros E m n_beta Ts T_R op_body Hfresh Hsafe m0 T U HT HU.
+  simpl in HT, HU.
+  destruct HT as [HT | HT]; destruct HU as [HU | HU].
+  - injection HT; injection HU; intros; subst. reflexivity.
+  - injection HT; intros; subst. exfalso. apply Hfresh.
+    eapply marker_annots_marker_in. exact HU.
+  - injection HU; intros; subst. exfalso. apply Hfresh.
+    eapply marker_annots_marker_in. exact HT.
+  - eapply Hsafe; eauto.
+Qed.
+
+Lemma marker_types_safe_handler_m_fresh : forall m T_B T_R body,
+  ~ In m (markers_in body) ->
+  marker_types_safe body ->
+  marker_types_safe (term_handler_m m T_B T_R body).
+Proof.
+  intros m T_B T_R body Hfresh Hsafe m0 T U HT HU.
+  simpl in HT, HU.
+  destruct HT as [HT | HT]; destruct HU as [HU | HU].
+  - injection HT; injection HU; intros; subst. reflexivity.
+  - injection HT; intros; subst. exfalso. apply Hfresh.
+    eapply marker_annots_marker_in. exact HU.
+  - injection HU; intros; subst. exfalso. apply Hfresh.
+    eapply marker_annots_marker_in. exact HT.
+  - eapply Hsafe; eauto.
+Qed.
+
+Lemma marker_types_safe_resume_fresh : forall m T_B T_R body,
+  ~ In m (markers_in body) ->
+  marker_types_safe body ->
+  marker_types_safe (term_resume m T_B T_R body).
+Proof.
+  intros m T_B T_R body Hfresh Hsafe m0 T U HT HU.
+  simpl in HT, HU.
+  destruct HT as [HT | HT]; destruct HU as [HU | HU].
+  - injection HT; injection HU; intros; subst. reflexivity.
+  - injection HT; intros; subst. exfalso. apply Hfresh.
+    eapply marker_annots_marker_in. exact HU.
+  - injection HU; intros; subst. exfalso. apply Hfresh.
+    eapply marker_annots_marker_in. exact HT.
+  - eapply Hsafe; eauto.
+Qed.
+
 Lemma marker_annots_ctor_focus_in : forall p vs t ts,
   In p (marker_annots t) ->
   In p (List.concat (List.map marker_annots (vs ++ t :: ts))).
@@ -932,6 +2817,131 @@ Proof.
   - apply List.in_or_app. right. apply IHE. exact Hin.
 Qed.
 
+Lemma marker_types_safe_handle_alloc_closed_from_no_local :
+  forall E E_tag n_beta Ts T_B T_R op_body body m,
+    ~ In m (markers_in (plug E (term_handle E_tag n_beta Ts T_B T_R op_body body))) ->
+    ty_ty_closed 0 T_R ->
+    ty_lt_closed 0 T_R ->
+    marker_annots_no_local (plug E (term_handle E_tag n_beta Ts T_B T_R op_body body)) ->
+    marker_types_safe (plug E (term_handle E_tag n_beta Ts T_B T_R op_body body)) ->
+    marker_types_safe
+      (plug E
+        (term_handler_m m T_B T_R
+          (subst_tm 0 (term_cap E_tag m n_beta Ts T_R op_body) body))).
+Proof.
+  intros E E_tag n_beta Ts T_B T_R op_body body m Hfresh HTy HLt Hnl Hsafe.
+  eapply marker_types_safe_handle_alloc_closed; try eassumption.
+  apply marker_annots_no_local_closed.
+  eapply marker_annots_no_local_incl; [|exact Hnl].
+  intros p Hp. apply marker_annots_plug_in. simpl. apply List.in_or_app. left. exact Hp.
+Qed.
+
+Lemma step_preserves_marker_types_safe_no_local_with_hard_cases :
+  forall t t',
+    t ==> t' ->
+    marker_annots_no_local t ->
+    marker_types_safe t ->
+    (forall E_tag m n_beta Ts T_B T_R op_body Ss v P,
+      value v -> pure_ectx_m m P ->
+      marker_annots_no_local
+        (term_handler_m m T_B T_R
+          (plug P (term_perform (term_cap E_tag m n_beta Ts T_R op_body) Ss v))) ->
+      incl
+        (marker_annots
+          (subst_list_tm [v; term_resume m T_B T_R (plug (shift_ectx_tm 1 0 P) (term_var 0))]
+            (subst_list_ty_in_tm Ss op_body)))
+        (marker_annots
+          (term_handler_m m T_B T_R
+            (plug P (term_perform (term_cap E_tag m n_beta Ts T_R op_body) Ss v))))) ->
+    (forall E E_tag n_beta Ts T_B T_R op_body body m,
+      ectx_wf E ->
+      ~ In m (markers_in (plug E (term_handle E_tag n_beta Ts T_B T_R op_body body))) ->
+      marker_annots_no_local (plug E (term_handle E_tag n_beta Ts T_B T_R op_body body)) ->
+      marker_types_safe (plug E (term_handle E_tag n_beta Ts T_B T_R op_body body)) ->
+      marker_types_safe
+        (plug E
+          (term_handler_m m T_B T_R
+            (subst_tm 0 (term_cap E_tag m n_beta Ts T_R op_body) body)))) ->
+    marker_types_safe t'.
+Proof.
+  intros t t' Hstep Hnl Hsafe Hperform Hhandle.
+  inversion Hstep as
+    [E r r' Hwf Hhead Heq1 Heq2
+    | E E_tag n_beta Ts T_B T_R op_body body m Hwf Hfresh Heq1 Heq2]; subst.
+  - assert (Hnl_r : marker_annots_no_local r).
+    { eapply marker_annots_no_local_incl.
+      - intros p Hp. apply marker_annots_plug_in. exact Hp.
+      - exact Hnl. }
+    pose proof (head_step_marker_annots_incl_no_local_with_perform
+      r r' Hhead Hnl_r Hperform) as Hincl.
+    eapply marker_types_safe_plug_replace_incl; [exact Hincl | exact Hsafe].
+  - eapply Hhandle; eauto.
+Qed.
+
+Lemma step_preserves_marker_types_safe_no_local_with_perform_and_handle_closed :
+  forall t t',
+    t ==> t' ->
+    marker_annots_no_local t ->
+    marker_types_safe t ->
+    (forall E_tag m n_beta Ts T_B T_R op_body Ss v P,
+      value v -> pure_ectx_m m P ->
+      marker_annots_no_local
+        (term_handler_m m T_B T_R
+          (plug P (term_perform (term_cap E_tag m n_beta Ts T_R op_body) Ss v))) ->
+      incl
+        (marker_annots
+          (subst_list_tm [v; term_resume m T_B T_R (plug (shift_ectx_tm 1 0 P) (term_var 0))]
+            (subst_list_ty_in_tm Ss op_body)))
+        (marker_annots
+          (term_handler_m m T_B T_R
+            (plug P (term_perform (term_cap E_tag m n_beta Ts T_R op_body) Ss v))))) ->
+    (forall E E_tag n_beta Ts T_B T_R op_body body (m : marker),
+      t = plug E (term_handle E_tag n_beta Ts T_B T_R op_body body) ->
+      ty_ty_closed 0 T_R /\ ty_lt_closed 0 T_R) ->
+    marker_types_safe t'.
+Proof.
+  intros t t' Hstep Hnl Hsafe Hperform Hhandle_closed.
+  inversion Hstep as
+    [E r r' Hwf Hhead Heq1 Heq2
+    | E E_tag n_beta Ts T_B T_R op_body body m Hwf Hfresh Heq1 Heq2]; subst.
+  - assert (Hnl_r : marker_annots_no_local r).
+    { eapply marker_annots_no_local_incl.
+      - intros p Hp. apply marker_annots_plug_in. exact Hp.
+      - exact Hnl. }
+    pose proof (head_step_marker_annots_incl_no_local_with_perform
+      r r' Hhead Hnl_r Hperform) as Hincl.
+    eapply marker_types_safe_plug_replace_incl; [exact Hincl | exact Hsafe].
+  - destruct (Hhandle_closed E E_tag n_beta Ts T_B T_R op_body body m eq_refl) as [HTy HLt].
+    eapply marker_types_safe_handle_alloc_closed_from_no_local; eauto.
+Qed.
+
+Lemma step_preserves_marker_types_safe_no_local_typed_with_perform :
+  forall Γ t t' T,
+    eval_ctx Γ ->
+    Γ ⊢ₜ t : T ->
+    t ==> t' ->
+    marker_annots_no_local t ->
+    marker_types_safe t ->
+    (forall E_tag m n_beta Ts T_B T_R op_body Ss v P,
+      value v -> pure_ectx_m m P ->
+      marker_annots_no_local
+        (term_handler_m m T_B T_R
+          (plug P (term_perform (term_cap E_tag m n_beta Ts T_R op_body) Ss v))) ->
+      incl
+        (marker_annots
+          (subst_list_tm [v; term_resume m T_B T_R (plug (shift_ectx_tm 1 0 P) (term_var 0))]
+            (subst_list_ty_in_tm Ss op_body)))
+        (marker_annots
+          (term_handler_m m T_B T_R
+            (plug P (term_perform (term_cap E_tag m n_beta Ts T_R op_body) Ss v))))) ->
+    marker_types_safe t'.
+Proof.
+  intros Γ t t' T Hec Hty Hstep Hnl Hsafe Hperform.
+  eapply step_preserves_marker_types_safe_no_local_with_perform_and_handle_closed; eauto.
+  intros E E_tag n_beta Ts T_B T_R op_body body m Heq. subst.
+  eapply handle_result_closed_from_plug_typing_for_markers; eauto.
+Qed.
+
 Lemma marker_types_ok_handler_perform_annotation_match :
   forall m T_B T_H E_tag n_beta Ts T_R op_body Ss v P,
     marker_types_safe
@@ -945,6 +2955,294 @@ Proof.
   - simpl. left. reflexivity.
   - simpl. right. apply marker_annots_plug_in.
     simpl. left. reflexivity.
+Qed.
+
+Lemma marker_annots_perform_reduct_incl_no_local :
+  forall E_tag m n_beta Ts T_B T_R op_body Ss v P,
+    marker_annots_no_local
+      (term_handler_m m T_B T_R
+        (plug P (term_perform (term_cap E_tag m n_beta Ts T_R op_body) Ss v))) ->
+    incl
+      (marker_annots
+        (subst_list_tm [v; term_resume m T_B T_R (plug (shift_ectx_tm 1 0 P) (term_var 0))]
+          (subst_list_ty_in_tm Ss op_body)))
+      (marker_annots
+        (term_handler_m m T_B T_R
+          (plug P (term_perform (term_cap E_tag m n_beta Ts T_R op_body) Ss v)))).
+Proof.
+  intros E_tag m n_beta Ts T_B T_R op_body Ss v P Hnl.
+  set (perform_redex := term_perform (term_cap E_tag m n_beta Ts T_R op_body) Ss v).
+  set (source := term_handler_m m T_B T_R (plug P perform_redex)).
+  set (resume := term_resume m T_B T_R (plug (shift_ectx_tm 1 0 P) (term_var 0))).
+  assert (HTRnl : no_local_ty T_R = true).
+  { unfold marker_annots_no_local in Hnl. subst source perform_redex resume. simpl in Hnl.
+    inversion Hnl as [|mt rest Hhead Htail]; subst. exact Hhead. }
+  assert (Hop_nl : marker_annots_no_local op_body).
+  { subst source perform_redex resume.
+    eapply marker_annots_no_local_incl; [|exact Hnl].
+    intros p Hp. simpl. right. apply marker_annots_plug_in.
+    simpl. right. apply List.in_or_app. left. exact Hp. }
+  assert (Hv_nl : marker_annots_no_local v).
+  { subst source perform_redex resume.
+    eapply marker_annots_no_local_incl; [|exact Hnl].
+    intros p Hp. simpl. right. apply marker_annots_plug_in.
+    simpl. right. apply List.in_or_app. right. exact Hp. }
+  assert (Hresume_nl : marker_annots_no_local resume).
+  { subst source perform_redex resume. unfold marker_annots_no_local. simpl. constructor.
+    - exact HTRnl.
+    - eapply marker_annots_no_local_incl; [|exact Hnl].
+      intros p Hp. simpl. right.
+      eapply marker_annots_shift_ectx_tm_plug_var_incl with (r := term_perform (term_cap E_tag m n_beta Ts T_R op_body) Ss v).
+      exact Hp. }
+  assert (Hvincl : incl (marker_annots v) (marker_annots source)).
+  { subst source perform_redex resume. intros p Hp. simpl. right. apply marker_annots_plug_in.
+    simpl. right. apply List.in_or_app. right. exact Hp. }
+  assert (Hopincl : incl (marker_annots op_body) (marker_annots source)).
+  { subst source perform_redex resume. intros p Hp. simpl. right. apply marker_annots_plug_in.
+    simpl. right. apply List.in_or_app. left. exact Hp. }
+  assert (Hresincl : incl (marker_annots resume) (marker_annots source)).
+  { subst source perform_redex resume. intros p Hp. simpl in Hp. destruct Hp as [Hp | Hp].
+    - simpl. left. exact Hp.
+    - simpl. right.
+      eapply marker_annots_shift_ectx_tm_plug_var_incl with (r := term_perform (term_cap E_tag m n_beta Ts T_R op_body) Ss v).
+      exact Hp. }
+  intros p Hp.
+  pose proof (marker_annots_subst_list_tm_no_local_incl
+    [v; resume] (subst_list_ty_in_tm Ss op_body)
+    (Forall_cons _ Hv_nl (Forall_cons _ Hresume_nl (Forall_nil _)))
+    (marker_annots_no_local_subst_list_ty_in_tm Ss op_body Hop_nl)
+    p Hp) as Hincl.
+  subst resume source perform_redex.
+  rewrite marker_annots_subst_list_ty_in_tm_no_local in Hincl by exact Hop_nl.
+  simpl in Hincl. repeat rewrite List.app_nil_r in Hincl.
+  repeat rewrite List.in_app_iff in Hincl.
+  destruct Hincl as [[HvIn | HresIn] | HopIn].
+  - apply Hvincl. exact HvIn.
+  - apply Hresincl. exact HresIn.
+  - apply Hopincl. exact HopIn.
+Qed.
+
+Lemma step_preserves_marker_types_safe_no_local_typed : forall Γ t t' T,
+  eval_ctx Γ -> marker_annots_no_local t -> marker_types_safe t -> Γ ⊢ₜ t : T ->
+  t ==> t' -> marker_types_safe t'.
+Proof.
+  intros Γ t t' T Hec Hnl Hsafe Hty Hstep.
+  eapply step_preserves_marker_types_safe_no_local_typed_with_perform; eauto.
+  intros E_tag m n_beta Ts T_B T_R op_body Ss v P Hval Hpure Hnl_redex.
+  apply marker_annots_perform_reduct_incl_no_local. exact Hnl_redex.
+Qed.
+
+Lemma head_step_marker_annots_incl_closed_with_perform :
+  forall r r',
+    r -->h r' ->
+    marker_annots_closed r ->
+    (forall E_tag m n_beta Ts T_B T_R op_body Ss v P,
+      value v -> pure_ectx_m m P ->
+      marker_annots_closed
+        (term_handler_m m T_B T_R
+          (plug P (term_perform (term_cap E_tag m n_beta Ts T_R op_body) Ss v))) ->
+      incl
+        (marker_annots
+          (subst_list_tm [v; term_resume m T_B T_R (plug (shift_ectx_tm 1 0 P) (term_var 0))]
+            (subst_list_ty_in_tm Ss op_body)))
+        (marker_annots
+          (term_handler_m m T_B T_R
+            (plug P (term_perform (term_cap E_tag m n_beta Ts T_R op_body) Ss v))))) ->
+    incl (marker_annots r') (marker_annots r).
+Proof.
+  intros r r' Hstep Hclosed Hperform.
+  inversion Hstep; subst.
+  - (* H_Beta *)
+    simpl in Hclosed. apply Forall_app in Hclosed as [_ Hv].
+    apply marker_annots_beta_incl_closed. exact Hv.
+  - (* H_TyBeta *)
+    apply marker_annots_tybeta_incl_closed. exact Hclosed.
+  - (* H_LtBeta *)
+    apply marker_annots_ltbeta_incl_closed. exact Hclosed.
+  - (* H_MatchYes *)
+    simpl in Hclosed. apply Forall_app in Hclosed as [Hvs Hyn].
+    apply Forall_app in Hyn as [Hyes _].
+    apply marker_annots_match_yes_incl_closed; assumption.
+  - (* H_MatchNo *)
+    apply marker_annots_match_no_incl.
+  - (* H_Return *)
+    apply marker_annots_return_incl.
+  - (* H_Perform *)
+    eapply Hperform; eauto.
+  - (* H_Resume *)
+    simpl in Hclosed. apply Forall_app in Hclosed as [_ Hv].
+    apply marker_annots_resume_incl_closed. exact Hv.
+Qed.
+
+Lemma step_preserves_marker_types_safe_closed_with_perform_and_handle_closed :
+  forall t t',
+    t ==> t' ->
+    marker_annots_closed t ->
+    marker_types_safe t ->
+    (forall E_tag m n_beta Ts T_B T_R op_body Ss v P,
+      value v -> pure_ectx_m m P ->
+      marker_annots_closed
+        (term_handler_m m T_B T_R
+          (plug P (term_perform (term_cap E_tag m n_beta Ts T_R op_body) Ss v))) ->
+      incl
+        (marker_annots
+          (subst_list_tm [v; term_resume m T_B T_R (plug (shift_ectx_tm 1 0 P) (term_var 0))]
+            (subst_list_ty_in_tm Ss op_body)))
+        (marker_annots
+          (term_handler_m m T_B T_R
+            (plug P (term_perform (term_cap E_tag m n_beta Ts T_R op_body) Ss v))))) ->
+    (forall E E_tag n_beta Ts T_B T_R op_body body (m : marker),
+      t = plug E (term_handle E_tag n_beta Ts T_B T_R op_body body) ->
+      ty_ty_closed 0 T_R /\ ty_lt_closed 0 T_R) ->
+    marker_types_safe t'.
+Proof.
+  intros t t' Hstep Hclosed Hsafe Hperform Hhandle_closed.
+  inversion Hstep as
+    [E r r' Hwf Hhead Heq1 Heq2
+    | E E_tag n_beta Ts T_B T_R op_body body m Hwf Hfresh Heq1 Heq2]; subst.
+  - assert (Hclosed_r : marker_annots_closed r).
+    { eapply marker_annots_closed_incl.
+      - intros p Hp. apply marker_annots_plug_in. exact Hp.
+      - exact Hclosed. }
+    pose proof (head_step_marker_annots_incl_closed_with_perform
+      r r' Hhead Hclosed_r Hperform) as Hincl.
+    eapply marker_types_safe_plug_replace_incl; [exact Hincl | exact Hsafe].
+  - destruct (Hhandle_closed E E_tag n_beta Ts T_B T_R op_body body m eq_refl) as [HTy HLt].
+    eapply marker_types_safe_handle_alloc_closed; eauto.
+    eapply marker_annots_closed_incl; [|exact Hclosed].
+    intros p Hp. apply marker_annots_plug_in. simpl. apply List.in_or_app. left. exact Hp.
+Qed.
+
+Lemma step_preserves_marker_types_safe_closed_typed_with_perform :
+  forall Γ t t' T,
+    eval_ctx Γ ->
+    Γ ⊢ₜ t : T ->
+    t ==> t' ->
+    marker_annots_closed t ->
+    marker_types_safe t ->
+    (forall E_tag m n_beta Ts T_B T_R op_body Ss v P,
+      value v -> pure_ectx_m m P ->
+      marker_annots_closed
+        (term_handler_m m T_B T_R
+          (plug P (term_perform (term_cap E_tag m n_beta Ts T_R op_body) Ss v))) ->
+      incl
+        (marker_annots
+          (subst_list_tm [v; term_resume m T_B T_R (plug (shift_ectx_tm 1 0 P) (term_var 0))]
+            (subst_list_ty_in_tm Ss op_body)))
+        (marker_annots
+          (term_handler_m m T_B T_R
+            (plug P (term_perform (term_cap E_tag m n_beta Ts T_R op_body) Ss v))))) ->
+    marker_types_safe t'.
+Proof.
+  intros Γ t t' T Hec Hty Hstep Hclosed Hsafe Hperform.
+  eapply step_preserves_marker_types_safe_closed_with_perform_and_handle_closed; eauto.
+  intros E E_tag n_beta Ts T_B T_R op_body body m Heq. subst.
+  eapply handle_result_closed_from_plug_typing_for_markers; eauto.
+Qed.
+
+Lemma marker_annots_perform_reduct_incl_closed :
+  forall E_tag m n_beta Ts T_B T_R op_body Ss v P,
+    marker_annots_closed
+      (term_handler_m m T_B T_R
+        (plug P (term_perform (term_cap E_tag m n_beta Ts T_R op_body) Ss v))) ->
+    incl
+      (marker_annots
+        (subst_list_tm [v; term_resume m T_B T_R (plug (shift_ectx_tm 1 0 P) (term_var 0))]
+          (subst_list_ty_in_tm Ss op_body)))
+      (marker_annots
+        (term_handler_m m T_B T_R
+          (plug P (term_perform (term_cap E_tag m n_beta Ts T_R op_body) Ss v)))).
+Proof.
+  intros E_tag m n_beta Ts T_B T_R op_body Ss v P Hclosed.
+  set (perform_redex := term_perform (term_cap E_tag m n_beta Ts T_R op_body) Ss v).
+  set (source := term_handler_m m T_B T_R (plug P perform_redex)).
+  set (resume := term_resume m T_B T_R (plug (shift_ectx_tm 1 0 P) (term_var 0))).
+  assert (HTRclosed : ty_ty_closed 0 T_R /\ ty_lt_closed 0 T_R).
+  { unfold marker_annots_closed in Hclosed. subst source perform_redex resume. simpl in Hclosed.
+    inversion Hclosed as [|mt rest Hhead Htail]; subst. exact Hhead. }
+  assert (Hop_closed : marker_annots_closed op_body).
+  { subst source perform_redex resume.
+    eapply marker_annots_closed_incl; [|exact Hclosed].
+    intros p Hp. simpl. right. apply marker_annots_plug_in.
+    simpl. right. apply List.in_or_app. left. exact Hp. }
+  assert (Hv_closed : marker_annots_closed v).
+  { subst source perform_redex resume.
+    eapply marker_annots_closed_incl; [|exact Hclosed].
+    intros p Hp. simpl. right. apply marker_annots_plug_in.
+    simpl. right. apply List.in_or_app. right. exact Hp. }
+  assert (Hresume_closed : marker_annots_closed resume).
+  { subst source perform_redex resume. unfold marker_annots_closed. simpl. constructor.
+    - exact HTRclosed.
+    - eapply marker_annots_closed_incl; [|exact Hclosed].
+      intros p Hp. simpl. right.
+      eapply marker_annots_shift_ectx_tm_plug_var_incl with (r := term_perform (term_cap E_tag m n_beta Ts T_R op_body) Ss v).
+      exact Hp. }
+  assert (Hvincl : incl (marker_annots v) (marker_annots source)).
+  { subst source perform_redex resume. intros p Hp. simpl. right. apply marker_annots_plug_in.
+    simpl. right. apply List.in_or_app. right. exact Hp. }
+  assert (Hopincl : incl (marker_annots op_body) (marker_annots source)).
+  { subst source perform_redex resume. intros p Hp. simpl. right. apply marker_annots_plug_in.
+    simpl. right. apply List.in_or_app. left. exact Hp. }
+  assert (Hresincl : incl (marker_annots resume) (marker_annots source)).
+  { subst source perform_redex resume. intros p Hp. simpl in Hp. destruct Hp as [Hp | Hp].
+    - simpl. left. exact Hp.
+    - simpl. right.
+      eapply marker_annots_shift_ectx_tm_plug_var_incl with (r := term_perform (term_cap E_tag m n_beta Ts T_R op_body) Ss v).
+      exact Hp. }
+  intros p Hp.
+  pose proof (marker_annots_subst_list_tm_closed_repl_incl
+    [v; resume] (subst_list_ty_in_tm Ss op_body)
+    (Forall_cons _ Hv_closed (Forall_cons _ Hresume_closed (Forall_nil _)))
+    p Hp) as Hincl.
+  subst resume source perform_redex.
+  rewrite marker_annots_subst_list_ty_in_tm_closed in Hincl by exact Hop_closed.
+  simpl in Hincl. repeat rewrite List.app_nil_r in Hincl.
+  repeat rewrite List.in_app_iff in Hincl.
+  destruct Hincl as [[HvIn | HresIn] | HopIn].
+  - apply Hvincl. exact HvIn.
+  - apply Hresincl. exact HresIn.
+  - apply Hopincl. exact HopIn.
+Qed.
+
+Lemma step_preserves_marker_types_safe_closed_typed : forall Γ t t' T,
+  eval_ctx Γ -> marker_annots_closed t -> marker_types_safe t -> Γ ⊢ₜ t : T ->
+  t ==> t' -> marker_types_safe t'.
+Proof.
+  intros Γ t t' T Hec Hclosed Hsafe Hty Hstep.
+  eapply step_preserves_marker_types_safe_closed_typed_with_perform; eauto.
+  intros E_tag m n_beta Ts T_B T_R op_body Ss v P Hval Hpure Hclosed_redex.
+  apply marker_annots_perform_reduct_incl_closed. exact Hclosed_redex.
+Qed.
+
+Lemma step_preserves_marker_annots_closed_typed : forall Γ t t' T,
+  eval_ctx Γ -> marker_annots_closed t -> Γ ⊢ₜ t : T ->
+  t ==> t' -> marker_annots_closed t'.
+Proof.
+  intros Γ t t' T Hec Hclosed Hty Hstep.
+  inversion Hstep as
+    [E r r' Hwf Hhead Heq1 Heq2
+    | E E_tag n_beta Ts T_B T_R op_body body m Hwf Hfresh Heq1 Heq2]; subst.
+  - assert (Hclosed_r : marker_annots_closed r).
+    { eapply marker_annots_closed_incl.
+      - intros p Hp. apply marker_annots_plug_in. exact Hp.
+      - exact Hclosed. }
+    pose proof (head_step_marker_annots_incl_closed_with_perform r r' Hhead Hclosed_r) as Hincl.
+    assert (Hred_incl : incl (marker_annots r') (marker_annots r)).
+    { apply Hincl. intros E_tag m n_beta Ts T_B T_R op_body Ss v P Hval Hpure Hclosed_redex.
+      apply marker_annots_perform_reduct_incl_closed. exact Hclosed_redex. }
+    eapply marker_annots_closed_incl.
+    + apply marker_annots_plug_replace_incl. exact Hred_incl.
+    + exact Hclosed.
+  - destruct (handle_result_closed_from_plug_typing_for_markers
+      Γ E E_tag n_beta Ts T_B T_R op_body body T Hec Hty) as [HTy HLt].
+    assert (Hop_closed : marker_annots_closed op_body).
+    { eapply marker_annots_closed_incl; [|exact Hclosed].
+      intros p Hp. apply marker_annots_plug_in. simpl. apply List.in_or_app. left. exact Hp. }
+    eapply marker_annots_closed_cons_incl with
+      (m := m) (T := T_R)
+      (source := plug E (term_handle E_tag n_beta Ts T_B T_R op_body body)); eauto.
+    apply marker_annots_plug_replace_incl_cons.
+    apply marker_annots_handle_alloc_redex_incl_closed; assumption.
 Qed.
 
 Lemma marker_ok_ctor_focus_inv : forall ms K l lts Ts vs t ts,
@@ -1067,12 +3365,6 @@ Proof.
   - (* cons *) intros u ts Hu Hts ms ms' Hi Hm. simpl in *.
     destruct Hm as [Ha Hb]. split; [eapply Hu | eapply Hts]; eauto.
 Qed.
-
-(* go_eq_map for subst_ty_in_tm (the other go_eq_map lemmas live upstream). *)
-Lemma subst_ty_in_tm_go_eq_map : forall var R ts,
-  (fix go ts := match ts with [] => [] | u :: rest => subst_ty_in_tm var R u :: go rest end) ts =
-  List.map (subst_ty_in_tm var R) ts.
-Proof. intros; induction ts; simpl; congruence. Qed.
 
 (* Closes every term_list_ind case EXCEPT the constructor case, for the      *)
 (* marker-invariance lemmas: shift/type-subst/lt-subst never touch markers.   *)
@@ -1303,6 +3595,15 @@ Proof.
     destruct Hm as [Ha Hb]. split; [eapply Hu | eapply Hts]; eauto.
 Qed.
 
+Lemma marker_ok_handler_return_no_cap : forall m T_B T_R v ms,
+  has_rt_cap v = false ->
+  marker_ok ms (term_handler_m m T_B T_R v) ->
+  marker_ok ms v.
+Proof.
+  intros m T_B T_R v ms Hcap Hok.
+  simpl in Hok. eapply marker_ok_strengthen_no_cap; eauto.
+Qed.
+
 (* ================================================================== *)
 (* AXIOM 5: marker_ok preservation for the handler-elimination head   *)
 (* steps (H_Return / H_Perform), whose redex is `term_handler_m m`.   *)
@@ -1415,16 +3716,3 @@ Proof.
     + eapply marker_ok_mono; [ apply incl_tl; apply incl_refl | exact Hbody ].
 Qed.
 
-(* ================================================================ *)
-(* AXIOM 6: marker_types_safe preservation under one step.  Type-     *)
-(* substituting head steps (H_TyBeta, H_LtBeta, H_MatchYes,           *)
-(* H_Perform) rewrite the *types* recorded in marker annotations, so  *)
-(* preservation of the no-conflict invariant (marker_types_ok) needs  *)
-(* that those annotation types are closed/consistent — a typing       *)
-(* invariant (capability confinement + marker-type regularity), not a *)
-(* structural fact.  Stated with the full typing premise (= the       *)
-(* type_soundness obligation) so it is sound.                          *)
-(* ================================================================ *)
-Axiom step_preserves_marker_types_safe : forall Γ t t' T,
-  eval_ctx Γ -> marker_ok [] t -> marker_types_safe t -> Γ ⊢ₜ t : T ->
-  t ==> t' -> marker_types_safe t'.
